Source/DafnyCore/Compilers/Rust/Dafny-compiler-rust.dfy
@@ -1,4 +1,7 @@
 include "../Dafny/AST.dfy"
+// Dafny to Rust compilation tenets:
+// - The Compiled Dafny AST should be minimal
+// - The generated code should look idiomatic and close to the original Dafny file if possible
 
 // Rust AST
 module RAST {
@@ -42,9 +45,9 @@ module RAST {
     ensures forall t <- s :: f(t) <= r
   {
     if |s| == 0 then 0 else
-      var i := f(s[0]);
-      var j := SeqToHeight(s[1..], f);
-      if i < j then j else i
+    var i := f(s[0]);
+    var j := SeqToHeight(s[1..], f);
+    if i < j then j else i
   }
   datatype ModDecl =
     | RawDecl(body: string)
@@ -86,9 +89,17 @@ module RAST {
     }
   }
 
+  datatype NamelessFormal =
+    NamelessFormal(visibility: VISIBILITY, tpe: Type)
+  {
+    function ToString(ind: string): string {
+      (if visibility == PUB then "pub " else "") + tpe.ToString(ind)
+    }
+  }
+
   datatype Formals =
     | NamedFormals(fields: seq<Formal>)
-    | NamelessFormals(types: seq<Type>)
+    | NamelessFormals(types: seq<NamelessFormal>)
   {
     function ToString(ind: string, newLine: bool): string {
       if NamedFormals? then
@@ -107,7 +118,7 @@ module RAST {
         assert NamelessFormals?;
         var separator := if newLine then ",\n" + ind + IND else ", ";
         "("+
-        SeqToString(types, (t: Type) => t.ToString(ind + IND), separator)
+        SeqToString(types, (t: NamelessFormal) => t.ToString(ind + IND), separator)
         +")"
     }
   }
@@ -138,26 +149,108 @@ module RAST {
     }
   }
 
+  type TypeParamConstraint = Type
+
   datatype TypeParam =
-    | RawTypeParam(content: string)
+    | RawTypeParam(content: string, constraints: seq<TypeParamConstraint>)
   {
     static function ToStringMultiple(typeParams: seq<TypeParam>, ind: string): string {
       if |typeParams| == 0 then "" else
-      "<" + SeqToString(typeParams, (t: TypeParam) => t.ToString(ind + IND), ",") + ">"
+      "<" + SeqToString(typeParams, (t: TypeParam) => t.ToString(ind + IND), ", ") + ">"
+    }
+    static function {:tailrecursion true} AddConstraintsMultiple(
+      typeParams: seq<TypeParam>, constraints: seq<TypeParamConstraint>
+    ): seq<TypeParam> {
+      if |typeParams| == 0 then []
+      else
+        [typeParams[0].AddConstraints(constraints)] + AddConstraintsMultiple(typeParams[1..], constraints)
+    }
+    function AddConstraints(constraints: seq<TypeParamConstraint>): TypeParam {
+      this.(constraints := this.constraints + constraints)
     }
     function ToString(ind: string): string {
-      content
+      content + (
+        if |constraints| == 0 then
+          ""
+        else
+          ": " + SeqToString(constraints, (t: TypeParamConstraint) requires t < this =>
+                               t.ToString(ind + IND), " + "))
     }
   }
+  const Self := Borrowed(SelfOwned)
+  const SelfMut := BorrowedMut(SelfOwned)
+  function Rc(underlying: Type): Type {
+    TypeApp("::std::rc::Rc", [underlying])
+  }
+  function RefCell(underlying: Type): Type {
+    TypeApp("::std::cell::RefCell", [underlying])
+  }
+  function Vec(underlying: Type): Type {
+    TypeApp("::std::vec::Vec", [underlying])
+  }
+  
+  const CloneTrait := RawType("Clone")
+  const DafnyPrintTrait := RawType("::dafny_runtime::DafnyPrint")
+  const DefaultTrait := RawType("::std::default::Default")
+  const StaticTrait := RawType("'static")
+
+  function RawType(content: string): Type {
+    TypeApp(content, [])
+  }
+
   datatype Type =
-    | Self | SelfOwned | SelfMut
-    | RawType(content: string)
+    | SelfOwned
+    | U8 | U16 | U32 | U64 | U128 | I8 | I16 | I32 | I64 | I128
+    | TypeApp(baseName: string, arguments: seq<Type>)
+    | Borrowed(underlying: Type)
+    | BorrowedMut(underlying: Type)
+    | ImplType(underlying: Type)
+    | DynType(underlying: Type)
+    | TupleType(arguments: seq<Type>)
+    | FnType(arguments: seq<Type>, returnType: Type)
+    | IntersectionType(left: Type, right: Type)
   {
     function ToString(ind: string): string {
-      if Self? then "&Self" else
-      if SelfOwned? then "Self" else
-      if SelfMut? then "&mut Self" else
-      content
+      match this {
+        case Borrowed(underlying) => "&" + underlying.ToString(ind)
+        case BorrowedMut(underlying) => "&mut " + underlying.ToString(ind)
+        case ImplType(underlying) => "impl " + underlying.ToString(ind)
+        case DynType(underlying) => "dyn " + underlying.ToString(ind)
+        case FnType(arguments, returnType) => 
+          "::std::ops::Fn("+
+            SeqToString(arguments, (arg: Type) requires arg < this =>
+              arg.ToString(ind + IND), ", ")
+          +") -> " + returnType.ToString(ind + IND)
+        case IntersectionType(left, right) =>
+          left.ToString(ind) + " + " + right.ToString(ind)
+        case TupleType(args) =>
+          (if args == [] then
+            "()"
+           else
+            "(" +
+            SeqToString(args, (arg: Type) requires arg < this => arg.ToString(ind + IND), ", ")
+            + ")")
+        case TypeApp(base, args) =>
+          base +
+          (if args == [] then
+            ""
+           else
+            "<" +
+            SeqToString(args, (arg: Type) requires arg < this => arg.ToString(ind + IND), ", ")
+            + ">")
+            
+        case SelfOwned() => "Self"
+        case U8() => "u8"
+        case U16() => "u16"
+        case U32() => "u32"
+        case U64() => "u64"
+        case U128() => "u128"
+        case I8() => "i8"
+        case I16() => "i16"
+        case I32() => "i32"
+        case I64() => "i64"
+        case I128() => "i128"
+      }
     }
   }
 
@@ -205,8 +298,8 @@ module RAST {
   {
     function ToString(ind: string): string {
       if name == "self" && tpe.SelfOwned? then name
-      else if name == "&self" && tpe.Self? then name
-      else if name == "&mut self" && tpe.SelfMut? then name
+      else if name == "&self" && tpe == Borrowed(SelfOwned) then name
+      else if name == "&mut self" && tpe == Borrowed(SelfMut) then name
       else
         name + ": " + tpe.ToString(ind)
     }
@@ -272,37 +365,133 @@ module RAST {
     if i < j then j else i
   }
 
+  datatype DeclareType = MUT | CONST
+
+  function RcNew(underlying: Expr): Expr {
+    Call(RawExpr("::std::rc::Rc::new"), [], [underlying])
+  }
+
   datatype Expr =
       RawExpr(content: string)
     | Match(matchee: Expr, cases: seq<MatchCase>)
     | StmtExpr(stmt: Expr, rhs: Expr)
     | Block(underlying: Expr)
     | StructBuild(name: string, assignments: seq<AssignIdentifier>)
+    | Tuple(arguments: seq<Expr>)
     | UnaryOp(op1: string, underlying: Expr, format: Format.UnOpFormat)
     | BinaryOp(op2: string, left: Expr, right: Expr, format2: Format.BinOpFormat)
+    | LiteralInt(value: string)
+    | ConversionNum(tpe: Type, underlying: Expr)
+    | DeclareVar(declareType: DeclareType, name: string, optType: Option<Type>, optRhs: Option<Expr>)
+    | AssignVar(name: string, rhs: Expr)
+    | IfExpr(cond: Expr, thn: Expr, els: Expr)
+    | Loop(optCond: Option<Expr>, underlying: Expr)
+    | For(name: string, range: Expr, body: Expr)
+    | Labelled(lbl: string, underlying: Expr)
+    | Break(optLbl: Option<string>)
+    | Continue(optLbl: Option<string>)
+    | Return(optExpr: Option<Expr>)
+    | Call(obj: Expr, typeParameters: seq<Type>, arguments: seq<Expr>)
+    | Borrow(underlying: Expr)
   {
+    predicate NoExtraSemicolonAfter() {
+      DeclareVar? || AssignVar? || Break? || Continue? || Return? || 
+        (RawExpr? && |content| > 0 && content[|content| - 1] == ';')
+    }
     function Height(): nat {
       match this {
+        case LiteralInt(_) => 1
+        case ConversionNum(_, underlying) => 1 + underlying.Height()
         case Match(matchee, cases) =>
           1 + max(matchee.Height(),
-            SeqToHeight(cases, (oneCase: MatchCase) 
-              requires oneCase < this
-            => oneCase.Height()))
+                  SeqToHeight(cases, (oneCase: MatchCase)
+                              requires oneCase < this
+                              => oneCase.Height()))
         case StmtExpr(stmt, rhs) =>
-          1 + max(stmt.Height(), rhs.Height())
+          var default := 1 + max(stmt.Height(), rhs.Height());
+          match this {
+            case StmtExpr(DeclareVar(mod, name, Some(tpe), None), StmtExpr(AssignVar(name2, rhs), last)) =>
+              if name == name2 then
+                1 + default
+              else default
+            case _ => default
+          }
+          
         case Block(underlying) =>
           1 + underlying.Height()
         case StructBuild(name, assignments) =>
           1 + SeqToHeight(assignments, (assignment: AssignIdentifier)
-                        requires assignment < this
-                        => assignment.Height())
+                          requires assignment < this
+                          => assignment.Height())
+        case Tuple(arguments) =>
+          1 + SeqToHeight(arguments, (argument: Expr)
+                          requires argument < this
+                          => argument.Height())
         // Special cases
         case UnaryOp(_, underlying, _) => 1 + underlying.Height()
 
         case BinaryOp(op, left, right, format) =>
           1 + max(left.Height(), right.Height())
+        case IfExpr(cond, thn, els) =>
+          1 + max(cond.Height(), max(thn.Height(), els.Height()))
+        case DeclareVar(declareType, name, tpe, expr) =>
+          1 + (match expr {
+            case Some(e) => e.Height()
+            case None => 0
+          })
+        case AssignVar(name, expr) =>
+          1 + expr.Height()
+        case Loop(optCond, underlying) =>
+          1 + if optCond.Some? then max(optCond.value.Height(), underlying.Height()) else underlying.Height()
+        case Labelled(lbl, underlying) =>
+          1 + underlying.Height()
+        case Break(_) => 1
+        case Continue(_) => 1
+        case For(name, range, body) =>
+          1 + max(range.Height(), body.Height())
+        case Return(optExpr) =>
+          if optExpr.Some? then 1 + optExpr.value.Height() else 1
+        case Call(obj, tpes, args) =>
+          1 + max(obj.Height(),
+                max(SeqToHeight(tpes, (tpe: Type) requires tpe < this => 1),
+                  SeqToHeight(args, (arg: Expr) requires arg < this => arg.Height())))
+        case Borrow(underlying) =>
+          1 + underlying.Height()
         case _ =>
+          assert RawExpr?;
           1
+      }
+    }
+
+    // Wish: Prove that Optimize() preserves semantics, if any
+    opaque function Optimize(): (r: Expr)
+      ensures this == r || r.Height() < this.Height()
+    {
+      match this {
+        case ConversionNum(tpe, expr) =>
+          if || tpe.U8? || tpe.U16? || tpe.U32? || tpe.U64? || tpe.U128?
+             || tpe.I8? || tpe.I16? || tpe.I32? || tpe.I64? || tpe.I128? then
+            match expr {
+              case LiteralInt(number) =>
+                RawExpr(number)
+              case _ => this
+            }
+          else
+            this
+        case StmtExpr(DeclareVar(mod, name, Some(tpe), None), StmtExpr(AssignVar(name2, rhs), last)) =>
+          if name == name2 then
+            var rewriting := StmtExpr(DeclareVar(mod, name, Some(tpe), Some(rhs)), last);
+            assert rewriting.Height() < this.Height() by {
+              assert StmtExpr(AssignVar(name2, rhs), last).Height() ==
+                1 + max(AssignVar(name2, rhs).Height(), last.Height()) ==
+                1 + max(1 + rhs.Height(), last.Height());
+              assert this.Height() == 2 + max(1, 1 + max(1 + rhs.Height(), last.Height()));
+              assert rewriting.Height() == 1 + max(1 + rhs.Height(), last.Height());
+            }
+            rewriting
+          else
+            this
+        case _ => this
       }
     }
 
@@ -310,55 +499,114 @@ module RAST {
     function ToString(ind: string): string
       decreases Height()
     {
-      match this {
+      match this.Optimize() {
+        case LiteralInt(number) =>
+          "::std::rc::Rc::new(::dafny_runtime::BigInt::parse_bytes(b\"" + number + "\", 10).unwrap())"
+        case ConversionNum(tpe, expr) =>
+          if || tpe.U8? || tpe.U16? || tpe.U32? || tpe.U64? || tpe.U128?
+             || tpe.I8? || tpe.I16? || tpe.I32? || tpe.I64? || tpe.I128? then
+            "num::ToPrimitive::to_"+tpe.ToString(ind)+"(" + expr.ToString(ind) + ").unwrap()"
+          else
+            "<b>Unsupported: Numeric conversion to " + tpe.ToString(ind) + "</b>"
         case Match(matchee, cases) =>
           "match " + matchee.ToString(ind + IND) + " {" +
-            SeqToString(cases,
-              (c: MatchCase) requires c.Height() < this.Height() =>
-                "\n" + ind + IND + c.ToString(ind + IND), ",") +
-            "\n" + ind + "}"
-        case StmtExpr(stmt, rhs) =>
-          stmt.ToString(ind) + ";\n" + ind + rhs.ToString(ind)
+          SeqToString(cases,
+                      (c: MatchCase) requires c.Height() < this.Height() =>
+                        "\n" + ind + IND + c.ToString(ind + IND), ",") +
+          "\n" + ind + "}"
+        case StmtExpr(stmt, rhs) => // They are built like StmtExpr(StmtExpr(StmtExpr(..., 1), 2), 3...)
+          if stmt == RawExpr("") then rhs.ToString(ind) else
+          stmt.ToString(ind) + (if stmt.NoExtraSemicolonAfter() then "" else ";") +
+          "\n" + ind + rhs.ToString(ind)
         case Block(underlying) =>
           "{\n" + ind + IND + underlying.ToString(ind + IND) + "\n" + ind + "}"
+        case IfExpr(cond, thn, els) =>
+          "if " + cond.ToString(ind + IND) + " {\n" + ind + IND + thn.ToString(ind + IND) +
+          "\n" + ind + "} else {\n" + ind + IND + els.ToString(ind + IND) + "\n" + ind + "}"
         case StructBuild(name, assignments) =>
           name + " {" +
-            SeqToString(assignments, (assignment: AssignIdentifier)
-                        requires assignment.Height() < this.Height()
-                        =>
-                          "\n" + ind + IND + assignment.ToString(ind + IND), ",") +
-            (if |assignments| > 0 then "\n" + ind else "") + "}"
-        
+          SeqToString(assignments, (assignment: AssignIdentifier)
+                      requires assignment.Height() < this.Height()
+                      =>
+                        "\n" + ind + IND + assignment.ToString(ind + IND), ",") +
+          (if |assignments| > 0 then "\n" + ind else "") + "}"
+        case Tuple(arguments) =>
+          "(" +
+          SeqToString(arguments, (arg: Expr)
+                      requires arg.Height() < this.Height()
+                      =>
+                        "\n" + ind + IND + arg.ToString(ind + IND), ",") +
+          (if |arguments| > 0 then "\n" + ind else "") + ")"
+
         // Special cases
         case UnaryOp("!", BinaryOp("==", left, right, format),
-            CombineNotInner()) =>
+          CombineNotInner()) =>
           assert BinaryOp("==", left, right, format).Height()
-            == BinaryOp("!=", left, right, BinOpFormat.NoFormat()).Height();
+              == BinaryOp("!=", left, right, BinOpFormat.NoFormat()).Height();
           BinaryOp("!=", left, right, BinOpFormat.NoFormat()).ToString(ind)
 
         case UnaryOp("!", BinaryOp("<", left, right, NoFormat()),
-            CombineNotInner()) =>
+          CombineNotInner()) =>
           assert BinaryOp(">=", left, right, BinOpFormat.NoFormat()).Height()
-            == BinaryOp("<", left, right, BinOpFormat.NoFormat()).Height();
+              == BinaryOp("<", left, right, BinOpFormat.NoFormat()).Height();
           BinaryOp(">=", left, right, BinOpFormat.NoFormat()).ToString(ind)
-        
+
         case UnaryOp("!", BinaryOp("<", left, right, ReverseOperands()),
-            CombineNotInner()) =>
+          CombineNotInner()) =>
           assert BinaryOp("<=", right, left, BinOpFormat.NoFormat()).Height()
-            == BinaryOp("<", left, right, BinOpFormat.ReverseOperands()).Height();
+              == BinaryOp("<", left, right, BinOpFormat.ReverseOperands()).Height();
           BinaryOp("<=", right, left, BinOpFormat.NoFormat()).ToString(ind)
-        
+
         case UnaryOp(op, underlying, format) =>
           op + "("  + underlying.ToString(ind) + ")"
 
-        case BinaryOp(op, left, right, format) =>
+        case BinaryOp(op2, left, right, format) =>
           "(" + left.ToString(ind) + ")" + op2 + "(" + right.ToString(ind) + ")"
-        case _ =>
-          assert RawExpr?; AddIndent(content, ind)
+        case DeclareVar(declareType, name, optType, optExpr) =>
+          "let " + (if declareType == MUT then "mut " else "") +
+          name + (if optType.Some? then ": " + optType.value.ToString(ind + IND) else "") +
+          (if optExpr.Some? then " = " + optExpr.value.ToString(ind + IND) else "") + ";"
+        case AssignVar(name, expr) =>
+          name + " = " + expr.ToString(ind + IND) + ";"
+        case Labelled(name, underlying) =>
+          "'" + name + ": " + underlying.ToString(ind)
+        case Break(optLbl) =>
+          match optLbl {
+            case Some(lbl) => "break '" + lbl + ";"
+            case None => "break;"
+          }
+        case Continue(optLbl) =>
+          match optLbl {
+            case Some(lbl) => "continue '" + lbl + ";"
+            case None => "continue;"
+          }
+        case Loop(optCond, underlying) =>
+          (match optCond {
+            case None => "loop"
+            case Some(c) => "while " + c.ToString(ind + IND)
+          }) + " {\n" + ind + IND + underlying.ToString(ind + IND) + "\n" + ind + "}"
+        case For(name, range, body) =>
+          "for "+ name +" in " + range.ToString(ind + IND) + " {\n" + ind + IND +
+          body.ToString(ind + IND) + "\n" + ind + "}"
+        case Return(optExpr) =>
+          "return" + (if optExpr.Some? then " " + optExpr.value.ToString(ind + IND) else "") + ";"
+        case Call(expr, tpes, args) =>
+          expr.ToString(ind) + (
+            if |tpes| == 0 then ""
+            else
+              "::<" + SeqToString(tpes, (tpe: Type) => tpe.ToString(ind + IND), ", ") +">"
+          ) + "("+SeqToString(args, (arg: Expr) requires arg.Height() < this.Height() => arg.ToString(ind + IND), ", ")+")"
+        case Borrow(underlying) =>
+          "&(" + underlying.ToString(ind) + ")"
+        case r =>
+          assert r.RawExpr?; AddIndent(r.content, ind)
       }
     }
     function Then(rhs2: Expr): Expr {
-      StmtExpr(this, rhs2)
+      if this.StmtExpr? then
+        StmtExpr(stmt, rhs.Then(rhs2))
+      else
+        StmtExpr(this, rhs2)
     }
   }
 
@@ -387,16 +635,12 @@ module RAST {
 module {:extern "DCOMP"} DCOMP {
   import opened DAST
   import Strings = Std.Strings
+  import Std
   import opened Std.Wrappers
   import R = RAST
   const IND := R.IND
   type Type = DAST.Type
   type Formal = DAST.Formal
-
-  function runtime(suffix: string): string {
-    "::dafny_runtime" + suffix
-  }
-  const DafnyErasable := runtime("::DafnyErasable")
 
   // List taken from https://doc.rust-lang.org/book/appendix-01-keywords.html
   const reserved_rust := {
@@ -526,44 +770,31 @@ module {:extern "DCOMP"} DCOMP {
         typeParamsSet: set<Type>,
         typeParams: seq<R.TypeParam>,
         constrainedTypeParams: seq<R.TypeParam>,
-        whereConstraints: string,
-        constrainedEraseParams: seq<R.TypeParam>,
-        unerasedParams: string,
-        erasedParams: string)
+        whereConstraints: string)
     {
       typeParamsSet := {};
       typeParams := [];
       constrainedTypeParams := [];
       whereConstraints := "";
-      constrainedEraseParams := [];
-      unerasedParams := "";
-      erasedParams := "";
       var tpI := 0;
 
       if |params| > 0 {
-        whereConstraints := " where ";
-        unerasedParams := "<";
-        erasedParams := "<";
         while tpI < |params| {
           var tp := params[tpI];
           typeParamsSet := typeParamsSet + {tp};
           var genTp := GenType(tp, false, false);
-          typeParams := typeParams + [R.RawTypeParam(genTp)];
-          var baseConstraints := ": ::dafny_runtime::DafnyErasable + ::dafny_runtime::DafnyUnerasable<" + genTp + "> + Clone + ::dafny_runtime::DafnyPrint + ::std::default::Default";
-          constrainedTypeParams := constrainedTypeParams + [R.RawTypeParam(genTp + baseConstraints + " + 'static")];
-          whereConstraints := whereConstraints + "<" + genTp + " as ::dafny_runtime::DafnyErasable>::Erased: ::std::cmp::PartialEq" + ", ";
-          constrainedEraseParams := constrainedEraseParams + [R.RawTypeParam(genTp + "__Erased" + ", " + genTp + baseConstraints + " + ::dafny_runtime::DafnyUnerasable<" + genTp + "__Erased> + 'static")];
-          unerasedParams := unerasedParams + genTp + "__Erased" + ", ";
-          erasedParams := erasedParams + genTp + "::Erased" + ", ";
+          typeParams := typeParams + [R.RawTypeParam(genTp.ToString(IND), [])];
           tpI := tpI + 1;
         }
-        unerasedParams := unerasedParams + ">";
-        erasedParams := erasedParams + ">";
       }
+      var baseConstraints := [R.CloneTrait, R.DafnyPrintTrait, R.StaticTrait];
+      constrainedTypeParams := R.TypeParam.AddConstraintsMultiple(
+        typeParams, baseConstraints
+      );
     }
 
     static method GenClass(c: Class, path: seq<Ident>) returns (s: seq<R.ModDecl>) {
-      var typeParamsSet, sTypeParams, sConstrainedTypeParams, whereConstraints, constrainedEraseParams, unerasedParams, erasedParams := GenTypeParameters(c.typeParams);
+      var typeParamsSet, sTypeParams, sConstrainedTypeParams, whereConstraints := GenTypeParameters(c.typeParams);
       var constrainedTypeParams := R.TypeParam.ToStringMultiple(sConstrainedTypeParams, R.IND + R.IND);
 
       var fields: seq<R.Formal> := [];
@@ -572,15 +803,15 @@ module {:extern "DCOMP"} DCOMP {
       while fieldI < |c.fields| {
         var field := c.fields[fieldI];
         var fieldType := GenType(field.formal.typ, false, false);
-        fields := fields + [R.Formal("pub " + escapeIdent(field.formal.name), R.RawType("::std::cell::RefCell<" + fieldType + ">"))];
+        fields := fields + [R.Formal("pub " + escapeIdent(field.formal.name), R.TypeApp("::std::cell::RefCell", [fieldType]))];
 
         match field.defaultValue {
           case Some(e) => {
-            var eStr, _, _, _ := GenExpr(e, None, [], true);
+            var eStr, _, _ := GenExpr(e, None, [], true);
             fieldInits := fieldInits + [
               R.AssignIdentifier(
                 escapeIdent(field.formal.name),
-                R.RawExpr("::std::cell::RefCell::new(" + eStr + ")"))];
+                R.RawExpr("::std::cell::RefCell::new(" + eStr.ToString(IND) + ")"))];
           }
           case None => {
             fieldInits := fieldInits + [
@@ -596,7 +827,7 @@ module {:extern "DCOMP"} DCOMP {
       var typeParamI := 0;
       while typeParamI < |c.typeParams| {
         var tpeGen := GenType(c.typeParams[typeParamI], false, false);
-        fields := fields + [R.Formal("_phantom_type_param_" + Strings.OfNat(typeParamI), R.RawType("::std::marker::PhantomData<" + tpeGen + ">"))];
+        fields := fields + [R.Formal("_phantom_type_param_" + Strings.OfNat(typeParamI), R.TypeApp("::std::marker::PhantomData", [tpeGen]))];
         fieldInits := fieldInits + [
           R.AssignIdentifier(
             "_phantom_type_param_" + Strings.OfNat(typeParamI),
@@ -606,7 +837,8 @@ module {:extern "DCOMP"} DCOMP {
       }
 
       var struct := R.Struct([], escapeIdent(c.name), sTypeParams, R.NamedFormals(fields));
-      var typeParams := R.TypeParam.ToStringMultiple(sTypeParams, R.IND + R.IND);
+      var typeParamsAsTypes := 
+        Std.Collections.Seq.Map((typeParam: R.TypeParam) => R.RawType(typeParam.content), sTypeParams);
 
       s := [R.StructDecl(struct)];
 
@@ -626,7 +858,7 @@ module {:extern "DCOMP"} DCOMP {
 
       var i := R.Impl(
         sConstrainedTypeParams,
-        R.RawType(escapeIdent(c.name) + typeParams),
+        R.TypeApp(escapeIdent(c.name), typeParamsAsTypes),
         whereConstraints,
         implBody
       );
@@ -648,8 +880,8 @@ module {:extern "DCOMP"} DCOMP {
               var x := R.ImplDecl(
                 R.ImplFor(
                   sConstrainedTypeParams,
-                  R.RawType(pathStr + typeArgs),
-                  R.RawType("::std::rc::Rc<" + genSelfPath + typeParams + ">"),
+                  R.TypeApp(pathStr, typeArgs),
+                  R.Rc(R.TypeApp(genSelfPath, typeParamsAsTypes)),
                   whereConstraints,
                   body
                 ));
@@ -663,8 +895,8 @@ module {:extern "DCOMP"} DCOMP {
 
       var d := R.ImplFor(
         sConstrainedTypeParams,
-        R.RawType("::std::default::Default"),
-        R.RawType(escapeIdent(c.name) + typeParams),
+        R.DefaultTrait,
+        R.TypeApp(escapeIdent(c.name), typeParamsAsTypes),
         whereConstraints,
         [R.FnDecl(
            R.PRIV,
@@ -678,8 +910,8 @@ module {:extern "DCOMP"} DCOMP {
       var p :=
         R.ImplFor(
           sConstrainedTypeParams,
-          R.RawType("::dafny_runtime::DafnyPrint"),
-          R.RawType(escapeIdent(c.name) + typeParams),
+          R.DafnyPrintTrait,
+          R.TypeApp(escapeIdent(c.name), typeParamsAsTypes),
           "",
           [R.FnDecl(
              R.PRIV,
@@ -696,7 +928,7 @@ module {:extern "DCOMP"} DCOMP {
       var pp := R.ImplFor(
         sTypeParams,
         R.RawType("::std::cmp::PartialEq"),
-        R.RawType(escapeIdent(c.name) + typeParams),
+        R.TypeApp(escapeIdent(c.name), typeParamsAsTypes),
         "",
         [R.FnDecl(
            R.PRIV,
@@ -710,96 +942,65 @@ module {:extern "DCOMP"} DCOMP {
       );
       var ptrPartialEqImpl := [R.ImplDecl(pp)];
 
-      var ii := R.ImplDecl(R.ImplFor(
-                             sConstrainedTypeParams,
-                             R.RawType("::dafny_runtime::DafnyErasable"),
-                             R.RawType(escapeIdent(c.name) + typeParams),
-                             "",
-                             [R.RawImplMember("type Erased = " + escapeIdent(c.name) + erasedParams + ";")]
-                           ));
-      var u := R.ImplDecl(R.ImplFor(
-                            sConstrainedTypeParams,
-                            R.RawType("::dafny_runtime::DafnyUnerasable<" + escapeIdent(c.name) + unerasedParams + ">"),
-                            R.RawType(escapeIdent(c.name) + typeParams),
-                            "", []
-                          ));
-      var identEraseImpls := [ii, u];
-
-      s := s + defaultImpl + printImpl + ptrPartialEqImpl + identEraseImpls;
+      s := s + defaultImpl + printImpl + ptrPartialEqImpl;
     }
 
     static method GenTrait(t: Trait, containingPath: seq<Ident>) returns (s: string) {
       var typeParamsSet := {};
-      var typeParams := "";
+      var typeParams := [];
       var tpI := 0;
       if |t.typeParams| > 0 {
-        typeParams := "<";
         while tpI < |t.typeParams| {
           var tp := t.typeParams[tpI];
           typeParamsSet := typeParamsSet + {tp};
           var genTp := GenType(tp, false, false);
-          typeParams := typeParams + genTp + ", ";
+          typeParams := typeParams + [genTp];
           tpI := tpI + 1;
         }
-        typeParams := typeParams + ">";
       }
 
       var fullPath := containingPath + [Ident.Ident(t.name)];
       var implBody, _ := GenClassImplBody(t.body, true, Type.Path(fullPath, [], ResolvedType.Trait(fullPath)), typeParamsSet);
       s :=
         R.TraitDecl(R.Trait(
-                      [], R.RawType(escapeIdent(t.name) + typeParams),
+                      [], R.TypeApp(escapeIdent(t.name), typeParams),
                       "",
                       implBody
                     )).ToString(IND);
     }
 
     static method GenNewtype(c: Newtype) returns (s: seq<R.ModDecl>) {
-      var typeParamsSet, sTypeParams, sConstrainedTypeParams, whereConstraints, _, _, _ := GenTypeParameters(c.typeParams);
-      var typeParams := R.TypeParam.ToStringMultiple(sTypeParams, R.IND + R.IND);
+      var typeParamsSet, sTypeParams, sConstrainedTypeParams, whereConstraints := GenTypeParameters(c.typeParams);
+      var typeParamsAsTypes := 
+        Std.Collections.Seq.Map((t: R.TypeParam) => R.RawType(t.content), sTypeParams);
       var constrainedTypeParams := R.TypeParam.ToStringMultiple(sConstrainedTypeParams, R.IND + R.IND);
 
-      var underlyingType := GenType(c.base, false, false);
-      s := [R.StructDecl(
-              R.Struct(
-                [
-                  R.RawAttribute("#[derive(Clone, PartialEq)]"),
-                  R.RawAttribute("#[repr(transparent)]")
-                ],
-                escapeIdent(c.name),
-                sTypeParams,
-                R.NamelessFormals([R.RawType("pub " + underlyingType)])
-              ))];
-      s := s +
-      [R.ImplDecl(R.ImplFor(
-                    sConstrainedTypeParams,
-                    R.RawType("::dafny_runtime::DafnyErasable"),
-                    R.RawType(escapeIdent(c.name) + typeParams),
-                    "",
-                    [R.RawImplMember("type Erased = " + underlyingType + ";")]
-                  ))];
-      s := s +
-      [R.ImplDecl(
-         R.ImplFor(
-           sConstrainedTypeParams,
-           R.RawType("::dafny_runtime::DafnyUnerasable<" + underlyingType + ">"),
-           R.RawType(escapeIdent(c.name) + typeParams),
-           "", []))];
-      s := s +
-      [R.ImplDecl(
-         R.ImplFor(
-           sConstrainedTypeParams,
-           R.RawType("::dafny_runtime::DafnyUnerasable<" + escapeIdent(c.name) + typeParams + ">"),
-           R.RawType(escapeIdent(c.name) + typeParams),
-           "", []))];
+      var underlyingType;
+      match NewtypeToRustType(c.base, c.range) {
+        case Some(v) =>
+          underlyingType := v;
+        case None =>
+          underlyingType := GenType(c.base, false, false);
+      }
+      s := [
+        R.StructDecl(
+          R.Struct(
+            [
+              R.RawAttribute("#[derive(Clone, PartialEq)]"),
+              R.RawAttribute("#[repr(transparent)]")
+            ],
+            escapeIdent(c.name),
+            sTypeParams,
+            R.NamelessFormals([R.NamelessFormal(R.PUB, underlyingType)])
+          ))];
 
       var fnBody := "";
 
       match c.witnessExpr {
         case Some(e) => {
           // TODO(shadaj): generate statements
-          var eStr, _, _, _ := GenExpr(e, None, [], true);
-          fnBody := fnBody + escapeIdent(c.name) + "(" + eStr + ")\n";
+          var eStr, _, _ := GenExpr(e, None, [], true);
+          fnBody := fnBody + escapeIdent(c.name) + "(" + eStr.ToString(IND) + ")\n";
         }
         case None => {
           fnBody := fnBody + escapeIdent(c.name) + "(::std::default::Default::default())";
@@ -818,15 +1019,15 @@ module {:extern "DCOMP"} DCOMP {
         R.ImplDecl(
           R.ImplFor(
             sConstrainedTypeParams,
-            R.RawType("::std::default::Default"),
-            R.RawType(escapeIdent(c.name) + typeParams),
+            R.DefaultTrait,
+            R.TypeApp(escapeIdent(c.name), typeParamsAsTypes),
             whereConstraints,
             [body]))];
       s := s + [
         R.ImplDecl(R.ImplFor(
                      sConstrainedTypeParams,
-                     R.RawType("::dafny_runtime::DafnyPrint"),
-                     R.RawType(escapeIdent(c.name) + typeParams),
+                     R.DafnyPrintTrait,
+                     R.TypeApp(escapeIdent(c.name), typeParamsAsTypes),
                      "",
                      [R.FnDecl(R.PRIV,
                                R.Fn("fmt_print", [],
@@ -840,9 +1041,9 @@ module {:extern "DCOMP"} DCOMP {
           R.ImplFor(
             sConstrainedTypeParams,
             R.RawType("::std::ops::Deref"),
-            R.RawType(escapeIdent(c.name) + typeParams),
+            R.TypeApp(escapeIdent(c.name), typeParamsAsTypes),
             "",
-            [R.RawImplMember("type Target = " + underlyingType + ";"),
+            [R.RawImplMember("type Target = " + underlyingType.ToString(IND) + ";"),
              R.FnDecl(
                R.PRIV,
                R.Fn("deref", [],
@@ -852,10 +1053,10 @@ module {:extern "DCOMP"} DCOMP {
     }
 
     static method GenDatatype(c: Datatype) returns (s: seq<R.ModDecl>) {
-      var typeParamsSet, sTypeParams, sConstrainedTypeParams, whereConstraints, sConstrainedEraseParams, unerasedParams, erasedParams := GenTypeParameters(c.typeParams);
-      var typeParams := R.TypeParam.ToStringMultiple(sTypeParams, IND + IND);
+      var typeParamsSet, sTypeParams, sConstrainedTypeParams, whereConstraints := GenTypeParameters(c.typeParams);
+      var typeParamsAsTypes := 
+        Std.Collections.Seq.Map((t: R.TypeParam) => R.RawType(t.content), sTypeParams);
       var constrainedTypeParams := R.TypeParam.ToStringMultiple(sConstrainedTypeParams, IND + IND);
-      var constrainedEraseParams := R.TypeParam.ToStringMultiple(sConstrainedEraseParams, IND);
 
       var ctors: seq<R.EnumCase> := [];
       var i := 0;
@@ -867,9 +1068,12 @@ module {:extern "DCOMP"} DCOMP {
           var formal := ctor.args[j];
           var formalType := GenType(formal.typ, false, false);
           if c.isCo {
-            ctorArgs := ctorArgs + [R.Formal(escapeIdent(formal.name), R.RawType("::dafny_runtime::LazyFieldWrapper<" + formalType + ">"))];
+            ctorArgs := ctorArgs + [
+              R.Formal(escapeIdent(formal.name),
+              R.TypeApp("::dafny_runtime::LazyFieldWrapper", [formalType]))];
           } else {
-            ctorArgs := ctorArgs + [R.Formal(escapeIdent(formal.name), R.RawType(formalType))];
+            ctorArgs := ctorArgs + [
+              R.Formal(escapeIdent(formal.name), formalType)];
           }
           j := j + 1;
         }
@@ -944,7 +1148,7 @@ module {:extern "DCOMP"} DCOMP {
                 R.PUB,
                 R.Fn(
                   escapeIdent(formal.name),
-                  [], [R.Formal.self], Some(R.RawType("&" + formalType )),
+                  [], [R.Formal.self], Some(R.Borrowed(formalType)),
                   "",
                   Some(methodBody)
                 ))];
@@ -960,11 +1164,12 @@ module {:extern "DCOMP"} DCOMP {
         var types: seq<R.Type> := [];
         while typeI < |c.typeParams| {
           var genTp := GenType(c.typeParams[typeI], false, false);
-          types := types + [R.RawType("::std::marker::PhantomData::<" + genTp + ">")];
+          types := types + [R.TypeApp("::std::marker::PhantomData::", [genTp])];
           typeI := typeI + 1;
         }
         ctors := ctors + [R.EnumCase("_PhantomVariant",
-                                     R.NamelessFormals(types)
+                                     R.NamelessFormals(Std.Collections.Seq.Map(
+                                      tpe => R.NamelessFormal(R.PRIV, tpe), types))
                           )];
       }
 
@@ -978,26 +1183,10 @@ module {:extern "DCOMP"} DCOMP {
          R.ImplDecl(
            R.Impl(
              sConstrainedTypeParams,
-             R.RawType(escapeIdent(c.name) + typeParams),
+             R.TypeApp(escapeIdent(c.name), typeParamsAsTypes),
              whereConstraints,
              implBody
            ))];
-
-      var identEraseImpls :=
-        [R.ImplDecl(
-           R.ImplFor(
-             sConstrainedTypeParams,
-             R.RawType("::dafny_runtime::DafnyErasable"),
-             R.RawType(escapeIdent(c.name) + typeParams),
-             "",
-             [R.RawImplMember("type Erased = " + escapeIdent(c.name) + erasedParams + ";")]
-           )),
-         R.ImplDecl(
-           R.ImplFor(
-             sConstrainedEraseParams,
-             R.RawType("::dafny_runtime::DafnyUnerasable<" + escapeIdent(c.name) + unerasedParams + ">"),
-             R.RawType(escapeIdent(c.name) + typeParams),
-             "", []))];
 
       i := 0;
       var printImplBodyCases: seq<R.MatchCase> := [];
@@ -1049,8 +1238,8 @@ module {:extern "DCOMP"} DCOMP {
         R.ImplDecl(
           R.ImplFor(
             sConstrainedTypeParams,
-            R.RawType("::dafny_runtime::DafnyPrint"),
-            R.RawType(escapeIdent(c.name) + typeParams),
+            R.DafnyPrintTrait,
+            R.TypeApp(escapeIdent(c.name), typeParamsAsTypes),
             "",
             [R.FnDecl(
                R.PRIV,
@@ -1074,12 +1263,16 @@ module {:extern "DCOMP"} DCOMP {
           ];
           i := i + 1;
         }
+        var defaultConstrainedTypeParams := R.TypeParam.AddConstraintsMultiple(
+          sTypeParams, [R.DefaultTrait]
+        );
+
         defaultImpl := [
           R.ImplDecl(
             R.ImplFor(
-              sConstrainedTypeParams,
-              R.RawType("::std::default::Default"),
-              R.RawType(escapeIdent(c.name) + typeParams),
+              defaultConstrainedTypeParams,
+              R.DefaultTrait,
+              R.TypeApp(escapeIdent(c.name), typeParamsAsTypes),
               "",
               [R.FnDecl(
                  R.PRIV,
@@ -1093,7 +1286,7 @@ module {:extern "DCOMP"} DCOMP {
             ))];
       }
 
-      s := enumBody + identEraseImpls + printImpl + defaultImpl;
+      s := enumBody + printImpl + defaultImpl;
     }
 
     static method GenPath(p: seq<Ident>) returns (s: string) {
@@ -1115,134 +1308,132 @@ module {:extern "DCOMP"} DCOMP {
       }
     }
 
-    static method GenTypeArgs(args: seq<Type>, inBinding: bool, inFn: bool) returns (s: string) {
-      s := "";
+    static method GenTypeArgs(args: seq<Type>, inBinding: bool, inFn: bool) returns (s: seq<R.Type>) {
+      s := [];
       if |args| > 0 {
-        s := s + "<";
         var i := 0;
         while i < |args| {
-          if i > 0 {
-            s := s + ", ";
-          }
-
           var genTp := GenType(args[i], inBinding, inFn);
-          s := s + genTp;
+          s := s + [genTp];
           i := i + 1;
         }
-        s := s + ">";
       }
     }
 
-    static method GenType(c: Type, inBinding: bool, inFn: bool) returns (s: string) {
+    static method GenType(c: Type, inBinding: bool, inFn: bool) returns (s: R.Type) {
       match c {
         case Path(p, args, resolved) => {
-          s := GenPath(p);
+          var t := GenPath(p);
+          s := R.TypeApp(t, []);
 
           var typeArgs := GenTypeArgs(args, inBinding, inFn);
-          s := s + typeArgs;
+          s := s.(arguments := typeArgs);
 
           match resolved {
             case Datatype(_) => {
-              s := "::std::rc::Rc<" + s + ">";
+              s := R.Rc(s);
             }
             case Trait(_) => {
               if p == [Ident.Ident("_System"), Ident.Ident("object")] {
-                s := "::std::rc::Rc<dyn ::std::any::Any>";
+                s := R.RawType("::std::rc::Rc<dyn ::std::any::Any>");
               } else {
                 if inBinding {
                   // impl trait in bindings is not stable
-                  s := "_";
+                  s := R.RawType("_");
                 } else {
-                  s := "impl " + s + "";
+                  s := R.ImplType(s);
                 }
               }
             }
-            case Primitive => {}
+            case Newtype(t, range, erased) => {
+              if erased {
+                match NewtypeToRustType(t, range) {
+                  case Some(v) =>
+                    s := v;
+                  case None =>
+                }
+              }
+            }
           }
         }
         case Nullable(inner) => {
-          var innerStr := GenType(inner, inBinding, inFn);
-          s := "::std::option::Option<" + innerStr + ">";
+          var innerExpr := GenType(inner, inBinding, inFn);
+          s := R.TypeApp("::std::option::Option", [innerExpr]);
         }
         case Tuple(types) => {
-          s := "(";
+          var args := [];
           var i := 0;
           while i < |types| {
-            if i > 0 {
-              s := s + " ";
-            }
-
             var generated := GenType(types[i], inBinding, inFn);
-            s := s + generated + ",";
+            args := args + [generated];
             i := i + 1;
           }
-
-          s := s + ")";
+          s := R.TupleType(args);
         }
         case Array(element, dims) => {
-          var elemStr := GenType(element, inBinding, inFn);
-          s := elemStr;
+          var elem := GenType(element, inBinding, inFn);
+          s := elem;
           var i := 0;
           while i < dims {
-            s := "::std::rc::Rc<::std::cell::RefCell<::std::vec::Vec<" + s + ">>>";
+            s := R.Rc(R.RefCell(R.Vec(s)));
             i := i + 1;
           }
         }
         case Seq(element) => {
-          var elemStr := GenType(element, inBinding, inFn);
-          s := "::std::vec::Vec<" + elemStr + ">";
+          var elem := GenType(element, inBinding, inFn);
+          s := R.Vec(elem);
         }
         case Set(element) => {
-          var elemStr := GenType(element, inBinding, inFn);
-          s := "::std::collections::HashSet<" + elemStr + ">";
+          var elem := GenType(element, inBinding, inFn);
+          s := R.TypeApp("::std::collections::HashSet", [elem]);
         }
         case Multiset(element) => {
-          var elemStr := GenType(element, inBinding, inFn);
-          s := "::std::collections::HashMap<" + elemStr + ", u64>";
+          var elem := GenType(element, inBinding, inFn);
+          s := R.TypeApp("::std::collections::HashMap", [elem, R.U64]);
         }
         case Map(key, value) => {
-          var keyStr := GenType(key, inBinding, inFn);
-          var valueStr := GenType(value, inBinding, inFn);
-          s := "::std::collections::HashMap<" + keyStr + ", " + valueStr + ">";
+          var keyType := GenType(key, inBinding, inFn);
+          var valueType := GenType(value, inBinding, inFn);
+          s := R.TypeApp("::std::collections::HashMap", [keyType, valueType]);
         }
         case Arrow(args, result) => {
           // we cannot use impl until Rc<Fn> impls Fn
           // if inFn || inBinding {
-          s := "::dafny_runtime::FunctionWrapper<::std::rc::Rc<dyn ::std::ops::Fn(";
+          //  s := "::dafny_runtime::FunctionWrapper<::std::rc::Rc<dyn ::std::ops::Fn(";
           // } else {
           //   s := "::dafny_runtime::FunctionWrapper<impl ::std::ops::Fn(";
           // }
-
+          var argTypes := [];
           var i := 0;
           while i < |args| {
-            if i > 0 {
-              s := s + ", ";
-            }
 
             var generated := GenType(args[i], inBinding, true);
-            s := s + "&" + generated;
+            argTypes := argTypes + [R.Borrowed(generated)];
             i := i + 1;
           }
 
           var resultType := GenType(result, inBinding, inFn || inBinding);
+          s := R.TypeApp(
+            "::dafny_runtime::FunctionWrapper",
+            [R.FnType(argTypes, R.IntersectionType(resultType, R.StaticTrait))]);
 
           // if inFn || inBinding {
-          s := s + ") -> " + resultType + " + 'static>>";
+          //s := s + ") -> " + resultType + " + 'static>>";
           // } else {
           //   s := s + ") -> " + resultType + " + Clone + 'static>";
           // }
         }
-        case TypeArg(Ident(name)) => s := escapeIdent(name);
+        case TypeArg(Ident(name)) => s := R.RawType(escapeIdent(name));
         case Primitive(p) => {
           match p {
-            case Int => s := "::dafny_runtime::BigInt";
-            case Real => s := "::dafny_runtime::BigRational";
-            case String => s := "Vec<char>";
-            case Bool => s := "bool";
-            case Char => s := "char";
+            case Int => s := R.Rc(R.RawType("::dafny_runtime::BigInt"));
+            case Real => s := R.Rc(R.RawType("::dafny_runtime::BigRational"));
+            case String => s := R.Vec(R.RawType("char"));
+            case Bool => s := R.RawType("bool");
+            case Char => s := R.RawType("char");
           }
         }
-        case Passthrough(v) => s := v;
+        case Passthrough(v) => s := R.RawType(v);
       }
     }
 
@@ -1285,7 +1476,7 @@ module {:extern "DCOMP"} DCOMP {
       while i < |params| {
         var param := params[i];
         var paramType := GenType(param.typ, false, false);
-        s := s + [R.Formal(escapeIdent(param.name), R.RawType(" &" + paramType))];
+        s := s + [R.Formal(escapeIdent(param.name), R.Borrowed(paramType))];
         i := i + 1;
       }
     }
@@ -1303,27 +1494,21 @@ module {:extern "DCOMP"} DCOMP {
         if (forTrait) {
           params := [R.Formal.self] + params;
         } else {
-          var enclosingTypeString := GenType(enclosingType, false, false);
-          params := [R.Formal("self", R.RawType("&" + enclosingTypeString))] + params;
+          var tpe := GenType(enclosingType, false, false);
+          params := [R.Formal("self", R.Borrowed(tpe))] + params;
         }
       }
 
-      var retType := if |m.outTypes| != 1 then "(" else "";
+      // TODO: Use mut instead of a tuple for the API of multiple output parameters
+      var retTypeArgs := [];
+      //var retType := if |m.outTypes| != 1 then "(" else "";
 
       var typeI := 0;
       while typeI < |m.outTypes| {
-        if typeI > 0 {
-          retType := retType + ", ";
-        }
-
-        var typeString := GenType(m.outTypes[typeI], false, false);
-        retType := retType + typeString;
+        var typeExpr := GenType(m.outTypes[typeI], false, false);
+        retTypeArgs := retTypeArgs + [typeExpr];
 
         typeI := typeI + 1;
-      }
-
-      if |m.outTypes| != 1 {
-        retType := retType + ")";
       }
 
       var visibility := R.PUB;//if forTrait then R.PUB else R.PRIV;
@@ -1349,15 +1534,15 @@ module {:extern "DCOMP"} DCOMP {
 
         var i := 0;
         while i < |typeParamsFiltered| {
-          if i > 0 {
-            whereClauses := whereClauses + ", ";
-          }
 
-          var typeString := GenType(typeParamsFiltered[i], false, false);
+          var typeExpr := GenType(typeParamsFiltered[i], false, false);
           typeParams := typeParams + [
-            R.RawTypeParam(typeString + ": ::dafny_runtime::DafnyErasable + ::dafny_runtime::DafnyUnerasable<" + typeString + "> + Clone + ::dafny_runtime::DafnyPrint + ::std::default::Default + 'static")
+            R.RawTypeParam(typeExpr.ToString(IND),
+                           [R.CloneTrait,
+                            R.DafnyPrintTrait,
+                            R.DefaultTrait,
+                            R.StaticTrait])
           ];
-          whereClauses := whereClauses + "<" + typeString + " as ::dafny_runtime::DafnyErasable>::Erased: ::std::cmp::PartialEq";
 
           i := i + 1;
         }
@@ -1366,29 +1551,28 @@ module {:extern "DCOMP"} DCOMP {
       var fBody: Option<R.Expr>;
 
       if m.hasBody {
-        var earlyReturn := "return;";
+        var earlyReturn: R.Expr := R.Return(None);
         match m.outVars {
           case Some(outVars) => {
-            earlyReturn := "return (";
+
+            var tupleArgs := [];
+
             var outI := 0;
             while outI < |outVars| {
-              if outI > 0 {
-                earlyReturn := earlyReturn + ", ";
-              }
 
               var outVar := outVars[outI];
-              earlyReturn := earlyReturn + escapeIdent(outVar.id);
+              tupleArgs := tupleArgs + [R.RawExpr(escapeIdent(outVar.id))];
 
               outI := outI + 1;
             }
-            earlyReturn := earlyReturn + ");";
+            earlyReturn := R.Return(Some(R.Tuple(tupleArgs)));
           }
           case None => {}
         }
 
         var body, _ := GenStmts(m.body, if m.isStatic then None else Some("self"), paramNames, true, earlyReturn);
 
-        fBody := Some(R.RawExpr(body));
+        fBody := Some(body);
       } else {
         fBody := None;
       }
@@ -1398,21 +1582,21 @@ module {:extern "DCOMP"} DCOMP {
           fnName,
           typeParams,
           params,
-          Some(R.RawType(retType)),
+          Some(if |retTypeArgs| == 1 then retTypeArgs[0] else R.TupleType(retTypeArgs)),
           whereClauses,
           fBody
         )
       );
     }
 
-    static method GenStmts(stmts: seq<Statement>, selfIdent: Option<string>, params: seq<string>, isLast: bool, earlyReturn: string) returns (generated: string, readIdents: set<string>) {
-      generated := "";
+    static method GenStmts(stmts: seq<Statement>, selfIdent: Option<string>, params: seq<string>, isLast: bool, earlyReturn: R.Expr) returns (generated: R.Expr, readIdents: set<string>) {
+      generated := R.RawExpr("");
       var declarations := {};
       readIdents := {};
       var i := 0;
       while i < |stmts| {
         var stmt := stmts[i];
-        var stmtString, recIdents := GenStmt(stmt, selfIdent, params, isLast && (i == |stmts| - 1), earlyReturn);
+        var stmtExpr, recIdents := GenStmt(stmt, selfIdent, params, isLast && (i == |stmts| - 1), earlyReturn);
         readIdents := readIdents + (recIdents - declarations);
 
         match stmt {
@@ -1421,12 +1605,8 @@ module {:extern "DCOMP"} DCOMP {
           }
           case _ => {}
         }
+        generated := generated.Then(stmtExpr);
 
-        if i > 0 {
-          generated := generated + "\n";
-        }
-
-        generated := generated + stmtString;
         i := i + 1;
       }
     }
@@ -1445,33 +1625,30 @@ module {:extern "DCOMP"} DCOMP {
         }
 
         case Select(on, field) => {
-          var onExpr, onOwned, onErased, recIdents := GenExpr(on, selfIdent, params, false);
-          generated := "*(" + onExpr + "." + field + ".borrow_mut()) = " + rhs + ";";
+          var onExpr, onOwned, recIdents := GenExpr(on, selfIdent, params, false);
+          generated := "*(" + onExpr.ToString(IND) + "." + field + ".borrow_mut()) = " + rhs + ";";
           readIdents := recIdents;
           needsIIFE := true;
         }
 
         case Index(on, indices) => {
-          var onExpr, onOwned, onErased, recIdents := GenExpr(on, selfIdent, params, false);
+          var onExpr, onOwned, recIdents := GenExpr(on, selfIdent, params, false);
           readIdents := recIdents;
 
           generated := "{\n";
 
           var i := 0;
           while i < |indices| {
-            var idx, _, idxErased, recIdentsIdx := GenExpr(indices[i], selfIdent, params, true);
-            if !idxErased {
-              idx := "::dafny_runtime::DafnyErasable::erase_owned(" + idx + ")";
-            }
+            var idx, _, recIdentsIdx := GenExpr(indices[i], selfIdent, params, true);
 
-            generated := generated + "let __idx" + Strings.OfNat(i) + " = <usize as ::dafny_runtime::NumCast>::from(" + idx + ").unwrap();\n";
+            generated := generated + "let __idx" + Strings.OfNat(i) + " = <usize as ::dafny_runtime::NumCast>::from(" + idx.ToString(IND) + ").unwrap();\n";
 
             readIdents := readIdents + recIdentsIdx;
 
             i := i + 1;
           }
 
-          generated := generated + onExpr + ".borrow_mut()";
+          generated := generated + onExpr.ToString(IND) + ".borrow_mut()";
           i := 0;
           while i < |indices| {
             generated := generated + "[__idx" + Strings.OfNat(i) + "]";
@@ -1484,121 +1661,106 @@ module {:extern "DCOMP"} DCOMP {
       }
     }
 
-    static method GenStmt(stmt: Statement, selfIdent: Option<string>, params: seq<string>, isLast: bool, earlyReturn: string) returns (generated: string, readIdents: set<string>) {
+    static method GenStmt(stmt: Statement, selfIdent: Option<string>, params: seq<string>, isLast: bool, earlyReturn: R.Expr) returns (generated: R.Expr, readIdents: set<string>) {
       match stmt {
         case DeclareVar(name, typ, Some(expression)) => {
           var typeString := GenType(typ, true, false);
-          var expr, _, recErased, recIdents := GenExpr(expression, selfIdent, params, true);
-          if !recErased {
-            expr := "::dafny_runtime::DafnyErasable::erase_owned(" + expr + ")";
-          }
+          var expr, _, recIdents := GenExpr(expression, selfIdent, params, true);
 
-          expr := "<" + typeString + " as ::dafny_runtime::DafnyUnerasable<_>>::unerase_owned(" + expr + ")";
-
-          generated := "let mut " + escapeIdent(name) + ": " + typeString + " = " + expr + ";";
+          generated := R.DeclareVar(R.MUT, escapeIdent(name), Some(typeString), Some(expr));
           readIdents := recIdents;
         }
         case DeclareVar(name, typ, None) => {
           var typeString := GenType(typ, true, false);
-          generated := "let mut " + escapeIdent(name) + ": " + typeString + ";";
+          generated := R.DeclareVar(R.MUT, escapeIdent(name), Some(typeString), None);
           readIdents := {};
         }
         case Assign(lhs, expression) => {
           var lhsGen, needsIIFE, recIdents := GenAssignLhs(lhs, "__rhs", selfIdent, params);
-          var exprGen, _, exprErased, exprIdents := GenExpr(expression, selfIdent, params, true);
-          if !exprErased {
-            exprGen := "::dafny_runtime::DafnyErasable::erase_owned(" + exprGen + ")";
-          }
-
-          exprGen := "::dafny_runtime::DafnyUnerasable::<_>::unerase_owned(" + exprGen + ")";
+          var exprGen, _, exprIdents := GenExpr(expression, selfIdent, params, true);
 
           if needsIIFE {
-            generated := "{\nlet __rhs = " + exprGen + ";\n" + lhsGen + "\n}";
+            generated := R.Block(
+              R.StmtExpr(
+                R.DeclareVar(R.CONST, "__rhs", None, Some(exprGen)),
+                R.RawExpr(lhsGen)
+              )
+            );
           } else {
-            generated := lhsGen + " = " + exprGen + ";";
+            generated := R.AssignVar(lhsGen, exprGen);
           }
 
           readIdents := recIdents + exprIdents;
         }
         case If(cond, thn, els) => {
-          var condString, _, condErased, recIdents := GenExpr(cond, selfIdent, params, true);
-          if !condErased {
-            condString := "::dafny_runtime::DafnyErasable::erase_owned(" + condString + ")";
-          }
+          var cond, _, recIdents := GenExpr(cond, selfIdent, params, true);
+          var condString := cond.ToString(IND);
 
           readIdents := recIdents;
-          var thnString, thnIdents := GenStmts(thn, selfIdent, params, isLast, earlyReturn);
+          var thn, thnIdents := GenStmts(thn, selfIdent, params, isLast, earlyReturn);
           readIdents := readIdents + thnIdents;
-          var elsString, elsIdents := GenStmts(els, selfIdent, params, isLast, earlyReturn);
+          var els, elsIdents := GenStmts(els, selfIdent, params, isLast, earlyReturn);
           readIdents := readIdents + elsIdents;
-          generated := "if " + condString + " {\n" + thnString + "\n} else {\n" + elsString + "\n}";
+          generated := R.IfExpr(cond, thn, els);
         }
         case Labeled(lbl, body) => {
-          var bodyString, bodyIdents := GenStmts(body, selfIdent, params, isLast, earlyReturn);
+          var body, bodyIdents := GenStmts(body, selfIdent, params, isLast, earlyReturn);
           readIdents := bodyIdents;
-          generated := "'label_" + lbl + ": loop {\n" + bodyString + "\n" + "break;" + "\n}";
+          generated := R.Labelled("label_" + lbl, R.Loop(None, R.StmtExpr(body, R.Break(None))));
         }
         case While(cond, body) => {
-          var condString, _, condErased, recIdents := GenExpr(cond, selfIdent, params, true);
-          if !condErased {
-            condString := "::dafny_runtime::DafnyErasable::erase_owned(" + condString + ")";
-          }
+          var cond, _, recIdents := GenExpr(cond, selfIdent, params, true);
 
           readIdents := recIdents;
-          var bodyString, bodyIdents := GenStmts(body, selfIdent, params, false, earlyReturn);
+          var body, bodyIdents := GenStmts(body, selfIdent, params, false, earlyReturn);
           readIdents := readIdents + bodyIdents;
 
-          generated := "while " + condString + " {\n" + bodyString + "\n}";
+          generated := R.Loop(Some(cond), body);
         }
         case Foreach(boundName, boundType, over, body) => {
-          var overString, _, overErased, recIdents := GenExpr(over, selfIdent, params, true);
+          var over, _, recIdents := GenExpr(over, selfIdent, params, true);
 
           var boundTypeStr := GenType(boundType, false, false);
 
           readIdents := recIdents;
-          var bodyString, bodyIdents := GenStmts(body, selfIdent, params + [boundName], false, earlyReturn);
+          var body, bodyIdents := GenStmts(body, selfIdent, params + [boundName], false, earlyReturn);
           readIdents := readIdents + bodyIdents - {boundName};
 
-          var unerasedIter := "_iter_erased";
-          if overErased {
-            unerasedIter := "<" + boundTypeStr + " as ::dafny_runtime::DafnyUnerasable<_>>::unerase_owned(" + unerasedIter + ")";
-          }
-
-          generated := "for _iter_erased in " + overString + " {\n";
-          generated := generated + "let " + escapeIdent(boundName) + " = " + unerasedIter + ";\n" + bodyString + "\n}";
+          generated := R.For(escapeIdent(boundName), over, body);
         }
         case Break(toLabel) => {
           match toLabel {
             case Some(lbl) => {
-              generated := "break 'label_" + lbl + ";";
+              generated := R.Break(Some("label_" + lbl));
             }
             case None => {
-              generated := "break;";
+              generated := R.Break(None);
             }
           }
           readIdents := {};
         }
         case TailRecursive(body) => {
           // clone the parameters to make them mutable
-          generated := "";
+          generated := R.RawExpr("");
 
           if selfIdent != None {
-            generated := generated + "let mut _this = self.clone();\n";
+            generated := generated.Then(R.DeclareVar(R.MUT, "_this", None, Some(R.RawExpr("self.clone()"))));
           }
 
           var paramI := 0;
           while paramI < |params| {
             var param := params[paramI];
-            generated := generated + "let mut " + escapeIdent(param) + " = " + escapeIdent(param) + ".clone();\n";
+            generated := generated.Then(R.DeclareVar(R.MUT, escapeIdent(param), None, Some(R.RawExpr(escapeIdent(param) + ".clone()"))));
             paramI := paramI + 1;
           }
 
-          var bodyString, bodyIdents := GenStmts(body, if selfIdent != None then Some("_this") else None, [], false, earlyReturn);
+          var body, bodyIdents := GenStmts(body, if selfIdent != None then Some("_this") else None, [], false, earlyReturn);
           readIdents := bodyIdents;
-          generated := generated + "'TAIL_CALL_START: loop {\n" + bodyString + "\n}";
+          generated := generated.Then(R.Labelled("TAIL_CALL_START", 
+            R.Loop(None, body)));
         }
         case JumpTailCallStart() => {
-          generated := "continue 'TAIL_CALL_START;";
+          generated := R.Continue(Some("TAIL_CALL_START"));
           readIdents := {};
         }
         case Call(on, name, typeArgs, args, maybeOutVars) => {
@@ -1607,18 +1769,14 @@ module {:extern "DCOMP"} DCOMP {
           var typeArgString := "";
           if (|typeArgs| >= 1) {
             var typeI := 0;
-            typeArgString := "::<";
+            var typeArgsR := [];
             while typeI < |typeArgs| {
-              if typeI > 0 {
-                typeArgString := typeArgString + ", ";
-              }
-
-              var typeString := GenType(typeArgs[typeI], false, false);
-              typeArgString := typeArgString + typeString;
+              var tpe := GenType(typeArgs[typeI], false, false);
+              typeArgsR := typeArgsR + [tpe];
 
               typeI := typeI + 1;
             }
-            typeArgString := typeArgString + ">";
+            typeArgString := R.TypeApp("::", typeArgsR).ToString(IND);
           }
 
           var argString := "";
@@ -1628,19 +1786,21 @@ module {:extern "DCOMP"} DCOMP {
               argString := argString + ", ";
             }
 
-            var argExpr, isOwned, argErased, argIdents := GenExpr(args[i], selfIdent, params, false);
+            var argExpr, isOwned, argIdents := GenExpr(args[i], selfIdent, params, false);
+            var argExprString := argExpr.ToString(IND);
             if isOwned {
-              argExpr := "&" + argExpr;
+              argExprString := "&" + argExprString;
             }
 
-            argString := argString + argExpr;
+            argString := argString + argExprString;
             readIdents := readIdents + argIdents;
 
             i := i + 1;
           }
 
-          var enclosingString, _, _, enclosingIdents := GenExpr(on, selfIdent, params, false);
+          var enclosingExpr, _, enclosingIdents := GenExpr(on, selfIdent, params, false);
           readIdents := readIdents + enclosingIdents;
+          var enclosingString := enclosingExpr.ToString(IND);
           match on {
             case Companion(_) => {
               enclosingString := enclosingString + "::";
@@ -1674,19 +1834,18 @@ module {:extern "DCOMP"} DCOMP {
             case None => {}
           }
 
-          generated :=
+          generated := R.RawExpr(
             (if receiver != "" then (receiver + " = ") else "") +
-            enclosingString + escapeIdent(name) + typeArgString + "(" + argString + ");";
+            enclosingString + escapeIdent(name) + typeArgString + "(" + argString + ");");
         }
         case Return(expr) => {
-          var exprString, _, recErased, recIdents := GenExpr(expr, selfIdent, params, true);
-          exprString := "::dafny_runtime::DafnyUnerasable::<_>::unerase_owned(::dafny_runtime::DafnyErasable::erase_owned(" + exprString + "))";
+          var expr, _, recIdents := GenExpr(expr, selfIdent, params, true);
           readIdents := recIdents;
 
           if isLast {
-            generated := exprString;
+            generated := expr;
           } else {
-            generated := "return " + exprString + ";";
+            generated := R.Return(Some(expr));
           }
         }
         case EarlyReturn() => {
@@ -1694,106 +1853,121 @@ module {:extern "DCOMP"} DCOMP {
           readIdents := {};
         }
         case Halt() => {
-          generated := "panic!(\"Halt\");";
+          generated := R.RawExpr("panic!(\"Halt\");");
           readIdents := {};
         }
         case Print(e) => {
-          var printedExpr, isOwned, _, recIdents := GenExpr(e, selfIdent, params, false);
+          var printedExpr, isOwned, recIdents := GenExpr(e, selfIdent, params, false);
+          var printedExprString := printedExpr.ToString(IND);
           if isOwned {
-            printedExpr := "&(" + printedExpr + ")";
+            printedExprString := "&(" + printedExprString + ")";
           }
-          generated := "print!(\"{}\", ::dafny_runtime::DafnyPrintWrapper(" + printedExpr + "));";
+          generated := R.RawExpr("print!(\"{}\", ::dafny_runtime::DafnyPrintWrapper(" + printedExprString + "));");
           readIdents := recIdents;
         }
       }
     }
 
-    static const OpTable: map<BinOp, string> := map[
-      Mod() := "%",
-      And() := "&&",
-      Or() := "||",
-      Div() := "/",
-      Lt() := "<",
-      Plus() := "+",
-      Minus() := "-",
-      Times() := "*",
-      BitwiseAnd() := "&",
-      BitwiseOr() := "|",
-      BitwiseXor() := "^",
-      BitwiseShiftRight() := ">>",
-      BitwiseShiftLeft() := "<<"
-    ]
+    static const OpTable: map<BinOp, string>
+    := 
+    map[
+        Mod() := "%",
+        And() := "&&",
+        Or() := "||",
+        Div() := "/",
+        Lt() := "<",
+        Plus() := "+",
+        Minus() := "-",
+        Times() := "*",
+        BitwiseAnd() := "&",
+        BitwiseOr() := "|",
+        BitwiseXor() := "^",
+        BitwiseShiftRight() := ">>",
+        BitwiseShiftLeft() := "<<"
+      ]
 
-    static method GenExpr(e: Expression, selfIdent: Option<string>, params: seq<string>, mustOwn: bool) returns (s: string, isOwned: bool, isErased: bool, readIdents: set<string>)
+    static function NewtypeToRustType(base: Type, range: NewtypeRange)
+      : Option<R.Type> {
+      match range {
+        case NoRange() => None
+        case U8() => Some(R.Type.U8)
+        case U16() => Some(R.Type.U16)
+        case U32() => Some(R.Type.U32)
+        case U64() => Some(R.Type.U64)
+        case U128() => Some(R.Type.U128)
+        case I8() => Some(R.Type.I8)
+        case I16() => Some(R.Type.I16)
+        case I32() => Some(R.Type.I32)
+        case I64() => Some(R.Type.I64)
+        case I128() => Some(R.Type.I128)
+        case _ => None
+      }
+    }
+
+    static method GenExpr(e: Expression, selfIdent: Option<string>, params: seq<string>, mustOwn: bool) returns (r: R.Expr, isOwned: bool, readIdents: set<string>)
       ensures mustOwn ==> isOwned
       decreases e {
       match e {
         case Literal(BoolLiteral(false)) => {
-          s := "false";
+          r := R.RawExpr("false");
           isOwned := true;
-          isErased := false;
           readIdents := {};
         }
         case Literal(BoolLiteral(true)) => {
-          s := "true";
+          r := R.RawExpr("true");
           isOwned := true;
-          isErased := false;
           readIdents := {};
         }
         case Literal(IntLiteral(i, t)) => {
           match t {
             case Primitive(Int) => {
-              s := "::dafny_runtime::BigInt::parse_bytes(b\"" + i + "\", 10).unwrap()";
+              r := R.LiteralInt(i);
             }
             case o => {
               var genType := GenType(o, false, false);
-              s := "(" + i + " as " + genType + ")";
+              r := R.RawExpr("(" + i + " as " + genType.ToString(IND) + ")");
             }
           }
 
           isOwned := true;
-          isErased := false;
           readIdents := {};
         }
         case Literal(DecLiteral(n, d, t)) => {
           match t {
             case Primitive(Real) => {
-              s := "::dafny_runtime::BigRational::new(::dafny_runtime::BigInt::parse_bytes(b\"" + n + "\", 10).unwrap(), ::dafny_runtime::BigInt::parse_bytes(b\"" + d + "\", 10).unwrap())";
+              r := R.RcNew(R.RawExpr("::dafny_runtime::BigRational::new(::dafny_runtime::BigInt::parse_bytes(b\"" + n + "\", 10).unwrap(), ::dafny_runtime::BigInt::parse_bytes(b\"" + d + "\", 10).unwrap())"));
             }
             case o => {
               var genType := GenType(o, false, false);
-              s := "((" + n + ".0 / " + d + ".0" + ") as " + genType + ")";
+              r := R.RawExpr("((" + n + ".0 / " + d + ".0" + ") as " + genType.ToString(IND) + ")");
             }
           }
 
           isOwned := true;
-          isErased := false;
           readIdents := {};
         }
         case Literal(StringLiteral(l)) => {
           // TODO(shadaj): handle unicode properly
-          s := "\"" + l + "\".chars().collect::<Vec<char>>()";
+          r := R.RawExpr("\"" + l + "\".chars().collect::<Vec<char>>()");
           isOwned := true;
-          isErased := false;
           readIdents := {};
         }
         case Literal(CharLiteral(c)) => {
-          s := "::std::primitive::char::from_u32(" + Strings.OfNat(c as nat) + ").unwrap()";
+          r := R.RawExpr("::std::primitive::char::from_u32(" + Strings.OfNat(c as nat) + ").unwrap()");
           isOwned := true;
-          isErased := false;
           readIdents := {};
         }
         case Literal(Null(tpe)) => {
+          // TODO: Mikael. Null will be std::ptr::null, not Option::None.
           var tpeGen := GenType(tpe, false, false);
-          s := "(None as " + tpeGen + ")";
+          r := R.RawExpr("(None as " + tpeGen.ToString(IND) + ")");
           isOwned := true;
-          isErased := false;
           readIdents := {};
         }
         case Ident(name) => {
-          s := escapeIdent(name);
-          if !(name in params) {
-            s := "(&" + s + ")";
+          var s := escapeIdent(name);
+          if !(name in params) { // TODO(mikael) have a table to know which names are borrowed
+            r := R.RawExpr("(&" + s + ")");
           }
 
           if mustOwn {
@@ -1802,26 +1976,25 @@ module {:extern "DCOMP"} DCOMP {
           } else {
             isOwned := false;
           }
-
-          isErased := false;
+          r := R.RawExpr(s);
 
           readIdents := {name};
         }
         case Companion(path) => {
-          s := GenPath(path);
+          var p := GenPath(path);
+          r := R.RawExpr(p);
           isOwned := true;
-          isErased := true;
           readIdents := {};
         }
         case InitializationValue(typ) => {
-          var typString := GenType(typ, false, false);
-          s := "<" + typString + " as std::default::Default>::default()";
+          // TODO (Mikael): Make InitializationValue disappear.
+          var typExpr := GenType(typ, false, false);
+          r := R.RawExpr("<" + typExpr.ToString(IND) + " as std::default::Default>::default()");
           isOwned := true;
-          isErased := false;
           readIdents := {};
         }
         case Tuple(values) => {
-          s := "(";
+          var s := "(";
           readIdents := {};
 
           var i := 0;
@@ -1830,37 +2003,32 @@ module {:extern "DCOMP"} DCOMP {
               s := s + " ";
             }
 
-            var recursiveGen, _, isErased, recIdents := GenExpr(values[i], selfIdent, params, true);
-            if isErased {
-              recursiveGen := "::dafny_runtime::DafnyUnerasable::<_>::unerase_owned(" + recursiveGen + ")";
-            }
+            var recursiveGen, _, recIdents := GenExpr(values[i], selfIdent, params, true);
 
-            s := s + recursiveGen + ",";
+            s := s + recursiveGen.ToString(IND) + ",";
             readIdents := readIdents + recIdents;
 
             i := i + 1;
           }
           s := s + ")";
+          r := R.RawExpr(s);
+
           isOwned := true;
-          isErased := false;
         }
         case New(path, typeArgs, args) => {
           var path := GenPath(path);
-          s := "::std::rc::Rc::new(" + path;
+          // TODO(Mikael) Use allocate(...) here.
+          var s := "::std::rc::Rc::new(" + path;
           if |typeArgs| > 0 {
-            s := s + "::<";
             var i := 0;
+            var typeExprs := [];
             while i < |typeArgs| {
-              if i > 0 {
-                s := s + "::";
-              }
-
-              var typeString := GenType(typeArgs[i], false, false);
-              s := s + typeString;
+              var typeExpr := GenType(typeArgs[i], false, false);
+              typeExprs := typeExprs + [typeExpr];
 
               i := i + 1;
             }
-            s := s + ">";
+            s := s + R.TypeApp("::", typeExprs).ToString(IND);
           }
           s := s + "::new(";
           readIdents := {};
@@ -1870,42 +2038,37 @@ module {:extern "DCOMP"} DCOMP {
               s := s + ", ";
             }
 
-            var recursiveGen, _, isErased, recIdents := GenExpr(args[i], selfIdent, params, true);
-            if isErased {
-              recursiveGen := "::dafny_runtime::DafnyUnerasable::<_>::unerase_owned(" + recursiveGen + ")";
-            }
-            s := s + recursiveGen;
+            var recursiveGen, _, recIdents := GenExpr(args[i], selfIdent, params, true);
+            s := s + recursiveGen.ToString(IND);
             readIdents := readIdents + recIdents;
 
             i := i + 1;
           }
           s := s + "))";
+          r := R.RawExpr(s);
           isOwned := true;
-          isErased := true;
         }
         case NewArray(dims, typ) => {
           var i := |dims| - 1;
           var genTyp := GenType(typ, false, false);
-          s := "<" + genTyp + " as ::std::default::Default>::default()";
+          // TODO (Mikael): Prevent arrays from being initialized without initialization code
+          var s := "<" + genTyp.ToString(IND) + " as ::std::default::Default>::default()";
           readIdents := {};
           while i >= 0 {
-            var recursiveGen, _, isErased, recIdents := GenExpr(dims[i], selfIdent, params, true);
-            if !isErased {
-              recursiveGen := "::dafny_runtime::DafnyErasable::erase_owned(" + recursiveGen + ")";
-            }
+            var recursiveGen, _, recIdents := GenExpr(dims[i], selfIdent, params, true);
 
-            s := "::std::rc::Rc::new(::std::cell::RefCell::new(vec![" + s + "; <usize as ::dafny_runtime::NumCast>::from(" + recursiveGen + ").unwrap()]))";
+            s := "::std::rc::Rc::new(::std::cell::RefCell::new(vec![" + s + "; <usize as ::dafny_runtime::NumCast>::from(" + recursiveGen.ToString(IND) + ").unwrap()]))";
             readIdents := readIdents + recIdents;
 
             i := i - 1;
           }
 
+          r := R.RawExpr(s);
           isOwned := true;
-          isErased := false;
         }
         case DatatypeValue(path, typeArgs, variant, isCo, values) => {
           var path := GenPath(path);
-          s := "::std::rc::Rc::new(" + path + "::";
+          var s := "::std::rc::Rc::new(" + path + "::";
           if |typeArgs| > 0 {
             s := s + "<";
             var i := 0;
@@ -1914,8 +2077,8 @@ module {:extern "DCOMP"} DCOMP {
                 s := s + ", ";
               }
 
-              var typeString := GenType(typeArgs[i], false, false);
-              s := s + typeString;
+              var typeExpr := GenType(typeArgs[i], false, false);
+              s := s + typeExpr.ToString(IND);
 
               i := i + 1;
             }
@@ -1933,11 +2096,7 @@ module {:extern "DCOMP"} DCOMP {
             }
 
             if isCo {
-              var recursiveGen, _, isErased, recIdents := GenExpr(value, selfIdent, [], true);
-              if !isErased {
-                recursiveGen := "::dafny_runtime::DafnyErasable::erase_owned(" + recursiveGen + ")";
-              }
-              recursiveGen := "::dafny_runtime::DafnyUnerasable::<_>::unerase_owned(" + recursiveGen + ")";
+              var recursiveGen, _, recIdents := GenExpr(value, selfIdent, [], true);
 
               readIdents := readIdents + recIdents;
               var allReadCloned := "";
@@ -1946,162 +2105,158 @@ module {:extern "DCOMP"} DCOMP {
                 allReadCloned := allReadCloned + "let " + escapeIdent(next) + " = " + escapeIdent(next) + ".clone();\n";
                 recIdents := recIdents - {next};
               }
-              s := s + escapeIdent(name) + ": ::dafny_runtime::LazyFieldWrapper(::dafny_runtime::Lazy::new(::std::boxed::Box::new({\n" + allReadCloned + "move || (" + recursiveGen + ")})))";
+              s := s + escapeIdent(name) + ": ::dafny_runtime::LazyFieldWrapper(::dafny_runtime::Lazy::new(::std::boxed::Box::new({\n" + allReadCloned + "move || (" + recursiveGen.ToString(IND) + ")})))";
             } else {
-              var recursiveGen, _, isErased, recIdents := GenExpr(value, selfIdent, params, true);
-              if !isErased {
-                recursiveGen := "::dafny_runtime::DafnyErasable::erase_owned(" + recursiveGen + ")";
-              }
-              recursiveGen := "::dafny_runtime::DafnyUnerasable::<_>::unerase_owned(" + recursiveGen + ")";
+              var recursiveGen, _, recIdents := GenExpr(value, selfIdent, params, true);
 
-              s := s + escapeIdent(name) + ": " + "(" + recursiveGen + ")";
+              s := s + escapeIdent(name) + ": " + "(" + recursiveGen.ToString(IND) + ")";
               readIdents := readIdents + recIdents;
             }
             i := i + 1;
           }
           s := s + " })";
+
+          r := R.RawExpr(s);
           isOwned := true;
-          isErased := false;
         }
         case Convert(expr, fromTpe, toTpe) => {
           assert {:split_here} true;
           if fromTpe == toTpe {
-            var recursiveGen, recOwned, recErased, recIdents := GenExpr(expr, selfIdent, params, mustOwn);
-            s := recursiveGen;
+            var recursiveGen, recOwned, recIdents := GenExpr(expr, selfIdent, params, mustOwn);
+            r := recursiveGen;
             isOwned := recOwned;
-            isErased := recErased;
             readIdents := recIdents;
           } else {
             match (fromTpe, toTpe) {
               case (Nullable(_), _) => {
-                var recursiveGen, recOwned, recErased, recIdents := GenExpr(expr, selfIdent, params, mustOwn);
+                var recursiveGen, recOwned, recIdents := GenExpr(expr, selfIdent, params, mustOwn);
+                var s := recursiveGen.ToString(IND);
                 if !recOwned {
-                  recursiveGen := recursiveGen + ".as_ref()";
+                  s := s + ".as_ref()";
                 }
 
-                s := recursiveGen + ".unwrap()";
+                s := s + ".unwrap()";
+                r := R.RawExpr(s);
                 isOwned := recOwned;
-                isErased := recErased;
                 readIdents := recIdents;
               }
               case (_, Nullable(_)) => {
-                var recursiveGen, recOwned, recErased, recIdents := GenExpr(expr, selfIdent, params, mustOwn);
+                var recursiveGen, recOwned, recIdents := GenExpr(expr, selfIdent, params, mustOwn);
+                var s := recursiveGen.ToString(IND);
                 if !recOwned {
-                  recursiveGen := recursiveGen + ".clone()";
+                  s := s + ".clone()";
                 }
 
-                s := "Some(" + recursiveGen + ")";
+                s := "Some(" + s + ")";
+                r := R.RawExpr(s);
                 isOwned := true;
-                isErased := recErased;
                 readIdents := recIdents;
               }
-              case (_, Path(_, _, Newtype(b))) => {
+              case (_, Path(_, _, Newtype(b, range, erase))) => {
                 if fromTpe == b {
-                  var recursiveGen, recOwned, recErased, recIdents := GenExpr(expr, selfIdent, params, mustOwn);
+                  var recursiveGen, recOwned, recIdents := GenExpr(expr, selfIdent, params, mustOwn);
 
-                  var rhsType := GenType(toTpe, true, false);
-
-                  var uneraseFn := if recOwned then "unerase_owned" else "unerase";
-                  s := "<" + rhsType + " as ::dafny_runtime::DafnyUnerasable<_>>::" + uneraseFn + "(" + recursiveGen + ")";
-                  isOwned := recOwned;
-                  isErased := false;
+                  var potentialRhsType := NewtypeToRustType(b, range);
+                  match potentialRhsType {
+                    case Some(v) =>
+                      r := R.ConversionNum(v, recursiveGen);
+                      isOwned := true;
+                    case None =>
+                      if erase {
+                        r := recursiveGen;
+                      } else {
+                        var rhsType := GenType(toTpe, true, false);
+                        r := R.RawExpr(rhsType.ToString(IND) + "(" + recursiveGen.ToString(IND) + ")");
+                      }
+                      isOwned := recOwned;
+                  }
                   readIdents := recIdents;
                 } else {
                   assume {:axiom} Convert(Convert(expr, fromTpe, b), b, toTpe) < e; // make termination go through
-                  s, isOwned, isErased, readIdents := GenExpr(Convert(Convert(expr, fromTpe, b), b, toTpe), selfIdent, params, mustOwn);
+                  r, isOwned, readIdents := GenExpr(Convert(Convert(expr, fromTpe, b), b, toTpe), selfIdent, params, mustOwn);
                 }
               }
-              case (Path(_, _, Newtype(b)), _) => {
+              case (Path(_, _, Newtype(b, range, erase)), _) => {
                 if b == toTpe {
-                  var recursiveGen, recOwned, recErased, recIdents := GenExpr(expr, selfIdent, params, mustOwn);
-                  var uneraseFn := if recOwned then "erase_owned" else "erase";
-                  s := "::dafny_runtime::DafnyErasable::" + uneraseFn + "(" + recursiveGen + ")";
+                  var recursiveGen, recOwned, recIdents := GenExpr(expr, selfIdent, params, mustOwn);
+                  if erase {
+                    r := recursiveGen;
+                  } else {
+                    r := R.RawExpr(recursiveGen.ToString(IND) + ".0");
+                  }
                   isOwned := recOwned;
-                  isErased := true;
                   readIdents := recIdents;
                 } else {
                   assume {:axiom} Convert(Convert(expr, fromTpe, b), b, toTpe) < e; // make termination go through
-                  s, isOwned, isErased, readIdents := GenExpr(Convert(Convert(expr, fromTpe, b), b, toTpe), selfIdent, params, mustOwn);
+                  r, isOwned, readIdents := GenExpr(Convert(Convert(expr, fromTpe, b), b, toTpe), selfIdent, params, mustOwn);
                 }
               }
               case (Primitive(Int), Primitive(Real)) => {
-                var recursiveGen, _, _, recIdents := GenExpr(expr, selfIdent, params, true);
-                s := "::dafny_runtime::BigRational::from_integer(" + recursiveGen + ")";
+                var recursiveGen, _, recIdents := GenExpr(expr, selfIdent, params, true);
+                r := R.RcNew(R.RawExpr("::dafny_runtime::BigRational::from_integer(" + recursiveGen.ToString(IND) + ")"));
                 isOwned := true;
-                isErased := true;
                 readIdents := recIdents;
               }
               case (Primitive(Real), Primitive(Int)) => {
-                var recursiveGen, _, _, recIdents := GenExpr(expr, selfIdent, params, false);
-                s := "::dafny_runtime::dafny_rational_to_int(" + recursiveGen + ")";
+                var recursiveGen, _, recIdents := GenExpr(expr, selfIdent, params, false);
+                r := R.RawExpr("::dafny_runtime::dafny_rational_to_int(" + recursiveGen.ToString(IND) + ")");
                 isOwned := true;
-                isErased := true;
                 readIdents := recIdents;
               }
               case (Primitive(Int), Passthrough(_)) => {
                 var rhsType := GenType(toTpe, true, false);
-                var recursiveGen, _, _, recIdents := GenExpr(expr, selfIdent, params, true);
-                s := "<" + rhsType + " as ::dafny_runtime::NumCast>::from(" + recursiveGen + ").unwrap()";
+                var recursiveGen, _, recIdents := GenExpr(expr, selfIdent, params, true);
+                r := R.RawExpr("<" + rhsType.ToString(IND) + " as ::dafny_runtime::NumCast>::from(" + recursiveGen.ToString(IND) + ").unwrap()");
                 isOwned := true;
-                isErased := true;
                 readIdents := recIdents;
               }
               case (Passthrough(_), Primitive(Int)) => {
                 var rhsType := GenType(fromTpe, true, false);
-                var recursiveGen, _, _, recIdents := GenExpr(expr, selfIdent, params, true);
-                s := "::dafny_runtime::BigInt::from(" + recursiveGen + ")";
+                var recursiveGen, _, recIdents := GenExpr(expr, selfIdent, params, true);
+                r := R.RcNew(R.RawExpr("::dafny_runtime::BigInt::from(" + recursiveGen.ToString(IND) + ")"));
                 isOwned := true;
-                isErased := true;
                 readIdents := recIdents;
               }
               case (Primitive(Int), Primitive(Char)) => {
                 var rhsType := GenType(toTpe, true, false);
-                var recursiveGen, _, _, recIdents := GenExpr(expr, selfIdent, params, true);
-                s := "char::from_u32(<u32 as ::dafny_runtime::NumCast>::from(" + recursiveGen + ").unwrap()).unwrap()";
+                var recursiveGen, _, recIdents := GenExpr(expr, selfIdent, params, true);
+                r := R.RawExpr("char::from_u32(<u32 as ::dafny_runtime::NumCast>::from(" + recursiveGen.ToString(IND) + ").unwrap()).unwrap()");
                 isOwned := true;
-                isErased := true;
                 readIdents := recIdents;
               }
               case (Primitive(Char), Primitive(Int)) => {
                 var rhsType := GenType(fromTpe, true, false);
-                var recursiveGen, _, _, recIdents := GenExpr(expr, selfIdent, params, true);
-                s := "::dafny_runtime::BigInt::from(" + recursiveGen + " as u32)";
+                var recursiveGen, _, recIdents := GenExpr(expr, selfIdent, params, true);
+                r := R.RcNew(R.RawExpr("::dafny_runtime::BigInt::from(" + recursiveGen.ToString(IND) + " as u32)"));
                 isOwned := true;
-                isErased := true;
                 readIdents := recIdents;
               }
               case (Passthrough(_), Passthrough(_)) => {
-                var recursiveGen, _, _, recIdents := GenExpr(expr, selfIdent, params, true);
+                var recursiveGen, _, recIdents := GenExpr(expr, selfIdent, params, true);
                 var toTpeGen := GenType(toTpe, true, false);
 
-                s := "((" + recursiveGen + ") as " + toTpeGen + ")";
+                r := R.RawExpr("((" + recursiveGen.ToString(IND) + ") as " + toTpeGen.ToString(IND) + ")");
 
                 isOwned := true;
-                isErased := true;
                 readIdents := recIdents;
               }
               case _ => {
-                var recursiveGen, recOwned, recErased, recIdents := GenExpr(expr, selfIdent, params, mustOwn);
-                s := "(" + recursiveGen + "/* conversion not yet implemented */)";
+                var recursiveGen, recOwned, recIdents := GenExpr(expr, selfIdent, params, mustOwn);
+                r := R.RawExpr("(" + recursiveGen.ToString(IND) + "/* conversion not yet implemented */)");
                 isOwned := recOwned;
-                isErased := recErased;
                 readIdents := recIdents;
               }
             }
           }
         }
         case SeqConstruct(length, expr) => {
-          var recursiveGen, _, eErased, recIdents := GenExpr(expr, selfIdent, params, true);
-          var lengthGen, _, lengthErased, lengthIdents := GenExpr(length, selfIdent, params, true);
-          if !lengthErased {
-            lengthGen := "::dafny_runtime::DafnyErasable::erase_owned(" + lengthGen + ")";
-          }
+          var recursiveGen, _, recIdents := GenExpr(expr, selfIdent, params, true);
+          var lengthGen, _, lengthIdents := GenExpr(length, selfIdent, params, true);
 
-          s := "{\nlet _initializer = " + recursiveGen + ";\n::dafny_runtime::integer_range(::dafny_runtime::Zero::zero(), " + lengthGen + ").map(|i| _initializer.0(&i)).collect::<Vec<_>>()\n}";
+          r := R.RawExpr("{\nlet _initializer = " + recursiveGen.ToString(IND) + ";\n::dafny_runtime::integer_range(::dafny_runtime::Zero::zero(), " + lengthGen.ToString(IND) + ").map(|i| _initializer.0(&i)).collect::<Vec<_>>()\n}");
 
           readIdents := recIdents + lengthIdents;
           isOwned := true;
-          isErased := eErased;
         }
         case SeqValue(exprs, typ) => {
           readIdents := {};
@@ -2109,78 +2264,66 @@ module {:extern "DCOMP"} DCOMP {
           var genTpe := GenType(typ, false, false);
 
           var i := 0;
-          s := "(vec![";
+          var s := "(vec![";
           i := 0;
           while i < |exprs| {
             if i > 0 {
               s := s + ", ";
             }
 
-            var recursiveGen, _, isErased, recIdents := GenExpr(exprs[i], selfIdent, params, true);
+            var recursiveGen, _, recIdents := GenExpr(exprs[i], selfIdent, params, true);
             readIdents := readIdents + recIdents;
 
-            if isErased {
-              recursiveGen := "::dafny_runtime::DafnyUnerasable::<_>::unerase_owned(" + recursiveGen + ")";
-            }
-
-            s := s + recursiveGen;
+            s := s + recursiveGen.ToString(IND);
             i := i + 1;
           }
-          s := s + "] as Vec<" + genTpe + ">)";
+          s := s + "] as Vec<" + genTpe.ToString(IND) + ">)";
+          r := R.RawExpr(s);
 
           isOwned := true;
-          isErased := false;
         }
         case SetValue(exprs) => {
           var generatedValues := [];
           readIdents := {};
           var i := 0;
-          var allErased := true;
           while i < |exprs| {
-            var recursiveGen, _, isErased, recIdents := GenExpr(exprs[i], selfIdent, params, true);
-            allErased := allErased && isErased;
+            var recursiveGen, _, recIdents := GenExpr(exprs[i], selfIdent, params, true);
 
-            generatedValues := generatedValues + [(recursiveGen, isErased)];
+            generatedValues := generatedValues + [recursiveGen];
             readIdents := readIdents + recIdents;
             i := i + 1;
           }
 
-          s := "vec![";
+          var s := "vec![";
           i := 0;
           while i < |generatedValues| {
             if i > 0 {
               s := s + ", ";
             }
 
-            var gen := generatedValues[i].0;
-            if generatedValues[i].1 && !allErased {
-              gen := "::dafny_runtime::DafnyUnerasable::<_>::unerase_owned(" + gen + ")";
-            }
-
-            s := s + gen;
+            var gen := generatedValues[i];
+            s := s + gen.ToString(IND);
             i := i + 1;
           }
           s := s + "].into_iter().collect::<std::collections::HashSet<_>>()";
+          r := R.RawExpr(s);
 
           isOwned := true;
-          isErased := allErased;
         }
         case MapValue(mapElems) => {
           var generatedValues := [];
           readIdents := {};
           var i := 0;
-          var allErased := true;
           while i < |mapElems| {
-            var recursiveGenKey, _, isErasedKey, recIdentsKey := GenExpr(mapElems[i].0, selfIdent, params, true);
-            var recursiveGenValue, _, isErasedValue, recIdentsValue := GenExpr(mapElems[i].1, selfIdent, params, true);
-            allErased := allErased && isErasedKey && isErasedValue;
+            var recursiveGenKey, _, recIdentsKey := GenExpr(mapElems[i].0, selfIdent, params, true);
+            var recursiveGenValue, _, recIdentsValue := GenExpr(mapElems[i].1, selfIdent, params, true);
 
-            generatedValues := generatedValues + [(recursiveGenKey, recursiveGenValue, isErasedKey, isErasedValue)];
+            generatedValues := generatedValues + [(recursiveGenKey, recursiveGenValue)];
             readIdents := readIdents + recIdentsKey + recIdentsValue;
             i := i + 1;
           }
 
-          s := "vec![";
+          var s := "vec![";
           i := 0;
           while i < |generatedValues| {
             if i > 0 {
@@ -2189,160 +2332,121 @@ module {:extern "DCOMP"} DCOMP {
 
             var genKey := generatedValues[i].0;
             var genValue := generatedValues[i].1;
-            if generatedValues[i].2 && !allErased {
-              genKey := "::dafny_runtime::DafnyUnerasable::<_>::unerase_owned(" + genKey + ")";
-            }
-            if generatedValues[i].3 && !allErased {
-              genValue := "::dafny_runtime::DafnyUnerasable::<_>::unerase_owned(" + genValue + ")";
-            }
 
-            s := s + "(" + genKey + ", " + genValue + ")";
+            s := s + "(" + genKey.ToString(IND) + ", " + genValue.ToString(IND) + ")";
             i := i + 1;
           }
           s := s + "].into_iter().collect::<std::collections::HashMap<_, _>>()";
+          r := R.RawExpr(s);
 
           isOwned := true;
-          isErased := allErased;
         }
         case This() => {
           match selfIdent {
             case Some(id) => {
               if mustOwn {
-                s := id + ".clone()";
+                r := R.RawExpr(id + ".clone()");
                 isOwned := true;
               } else {
                 if id == "self" {
-                  s := "self";
+                  r := R.RawExpr("self");
                 } else {
-                  s := "&" + id;
+                  r := R.RawExpr("&" + id);
                 }
                 isOwned := false;
               }
 
               readIdents := {id};
-              isErased := false;
             }
             case None => {
-              s := "panic!(\"this outside of a method\")";
+              r := R.RawExpr("panic!(\"this outside of a method\")");
               isOwned := true;
               readIdents := {};
-              isErased := true;
             }
           }
         }
         case Ite(cond, t, f) => {
           assert {:split_here} true;
-          var condString, _, condErased, recIdentsCond := GenExpr(cond, selfIdent, params, true);
-          if !condErased {
-            condString := "::dafny_runtime::DafnyErasable::erase_owned(" + condString + ")";
-          }
+          var cond, _, recIdentsCond := GenExpr(cond, selfIdent, params, true);
+          var condString := cond.ToString(IND);
 
-          var _, tHasToBeOwned, _, _ := GenExpr(t, selfIdent, params, mustOwn); // check if t has to be owned even if not requested
-          var fString, fOwned, fErased, recIdentsF := GenExpr(f, selfIdent, params, tHasToBeOwned);
-          var tString, _, tErased, recIdentsT := GenExpr(t, selfIdent, params, fOwned); // there's a chance that f forced ownership
+          var _, tHasToBeOwned, _ := GenExpr(t, selfIdent, params, mustOwn); // check if t has to be owned even if not requested
+          var fExpr, fOwned, recIdentsF := GenExpr(f, selfIdent, params, tHasToBeOwned);
+          var fString := fExpr.ToString(IND);
+          var tExpr, _, recIdentsT := GenExpr(t, selfIdent, params, fOwned); // there's a chance that f forced ownership
+          var tString := tExpr.ToString(IND);
 
-          if !fErased || !tErased {
-            if fErased {
-              fString := "::dafny_runtime::DafnyErasable::erase_owned(" + fString + ")";
-            }
-
-            if tErased {
-              tString := "::dafny_runtime::DafnyErasable::erase_owned(" + tString + ")";
-            }
-          }
-
-          s := "(if " + condString + " {\n" + tString + "\n} else {\n" + fString + "\n})";
+          r := R.RawExpr("(if " + condString + " {\n" + tString + "\n} else {\n" + fString + "\n})");
           isOwned := fOwned;
           readIdents := recIdentsCond + recIdentsT + recIdentsF;
-          isErased := fErased || tErased;
         }
         case UnOp(Not, e, format) => {
-          var recursiveGen, _, recErased, recIdents := GenExpr(e, selfIdent, params, true);
-          if !recErased {
-            recursiveGen := "::dafny_runtime::DafnyErasable::erase_owned(" + recursiveGen + ")";
-          }
+          var recursiveGen, _, recIdents := GenExpr(e, selfIdent, params, true);
 
-          s := "!(" + recursiveGen + ")";
+          r := R.RawExpr("!(" + recursiveGen.ToString(IND) + ")");
           isOwned := true;
           readIdents := recIdents;
-          isErased := true;
         }
         case UnOp(BitwiseNot, e, format) => {
-          var recursiveGen, _, recErased, recIdents := GenExpr(e, selfIdent, params, true);
-          if !recErased {
-            recursiveGen := "::dafny_runtime::DafnyErasable::erase_owned(" + recursiveGen + ")";
-          }
+          var recursiveGen, _, recIdents := GenExpr(e, selfIdent, params, true);
 
-          s := "~(" + recursiveGen + ")";
+          r := R.RawExpr("~(" + recursiveGen.ToString(IND) + ")");
           isOwned := true;
           readIdents := recIdents;
-          isErased := true;
         }
         case UnOp(Cardinality, e, format) => {
-          var recursiveGen, recOwned, recErased, recIdents := GenExpr(e, selfIdent, params, false);
-          if !recErased {
-            var eraseFn := if recOwned then "erase_owned" else "erase";
-            recursiveGen := "::dafny_runtime::DafnyErasable::" + eraseFn + "(" + recursiveGen + ")";
-          }
+          var recursiveGen, recOwned, recIdents := GenExpr(e, selfIdent, params, false);
 
-          s := "::dafny_runtime::BigInt::from((" + recursiveGen + ").len())";
+          r := R.RcNew(R.RawExpr("::dafny_runtime::BigInt::from((" + recursiveGen.ToString(IND) + ").len())"));
           isOwned := true;
           readIdents := recIdents;
-          isErased := true;
         }
-        case BinOp(op, l, r, format) => {
-          var left, _, leftErased, recIdentsL := GenExpr(l, selfIdent, params, true);
-          var right, _, rightErased, recIdentsR := GenExpr(r, selfIdent, params, true);
+        case BinOp(op, lExpr, rExpr, format) => {
+          var left, _, recIdentsL := GenExpr(lExpr, selfIdent, params, true);
+          var right, _, recIdentsR := GenExpr(rExpr, selfIdent, params, true);
 
           match op {
             case In() => {
-              s := right + ".contains(&" + left + ")";
+              r := R.RawExpr(right.ToString(IND) + ".contains(&" + left.ToString(IND) + ")");
             }
             case SetDifference() => {
-              s := left + ".difference(&" + right + ").cloned().collect::<::std::collections::HashSet<_>>()";
+              r := R.RawExpr(left.ToString(IND) + ".difference(&" + right.ToString(IND) + ").cloned().collect::<::std::collections::HashSet<_>>()");
             }
             case Concat() => {
-              s := "[" + left + ", " + right + "].concat()";
+              r := R.RawExpr("[" + left.ToString(IND) + ", " + right.ToString(IND) + "].concat()");
             }
             case _ => {
-              if !leftErased {
-                left := "::dafny_runtime::DafnyErasable::erase_owned(" + left + ")";
-              }
-
-              if !rightErased {
-                right := "::dafny_runtime::DafnyErasable::erase_owned(" + right + ")";
-              }
 
               if op in OpTable {
-                s := R.Expr.BinaryOp(OpTable[op], 
-                    R.Expr.RawExpr(left),
-                    R.Expr.RawExpr(right),
-                    format).ToString("");
+                r := R.Expr.BinaryOp(OpTable[op],
+                                     left,
+                                     right,
+                                     format);
               } else {
                 match op {
                   case Eq(referential, nullable) => {
                     if (referential) {
                       // TODO: Render using a call with two expressions
                       if (nullable) {
-                        s := "::dafny_runtime::nullable_referential_equality(" + left + ", " + right + ")";
+                        r := R.RawExpr("::dafny_runtime::nullable_referential_equality(" + left.ToString(IND) + ", " + right.ToString(IND) + ")");
                       } else {
-                        s := "::std::rc::Rc::ptr_eq(&(" + left + "), &(" + right + "))";
+                        r := R.RawExpr("::std::rc::Rc::ptr_eq(&(" + left.ToString(IND) + "), &(" + right.ToString(IND) + "))");
                       }
                     } else {
-                      s := left + " == " + right;
+                      r := R.RawExpr(left.ToString(IND) + " == " + right.ToString(IND));
                     }
                   }
                   case EuclidianDiv() => {
-                    s := "::dafny_runtime::euclidian_division(" + left + ", " + right + ")";
+                    r := R.RawExpr("::dafny_runtime::euclidian_division(" + left.ToString(IND) + ", " + right.ToString(IND) + ")");
                   }
                   case EuclidianMod() => {
-                    s := "::dafny_runtime::euclidian_modulo(" + left + ", " + right + ")";
+                    r := R.RawExpr("::dafny_runtime::euclidian_modulo(" + left.ToString(IND) + ", " + right.ToString(IND) + ")");
                   }
                   case Passthrough(op) => {
-                    s := R.Expr.BinaryOp(op, 
-                      R.Expr.RawExpr(left),
-                      R.Expr.RawExpr(right),
-                      format).ToString("");
+                    r := R.Expr.BinaryOp(op,
+                                         left,
+                                         right,
+                                         format);
                   }
                 }
               }
@@ -2351,30 +2455,30 @@ module {:extern "DCOMP"} DCOMP {
 
           isOwned := true;
           readIdents := recIdentsL + recIdentsR;
-          isErased := true;
         }
         case ArrayLen(expr, dim) => {
-          var recursiveGen, _, recErased, recIdents := GenExpr(expr, selfIdent, params, true);
+          var recursiveGen, _, recIdents := GenExpr(expr, selfIdent, params, true);
 
           if dim == 0 {
-            s := "::dafny_runtime::BigInt::from((" + recursiveGen + ").borrow().len())";
+            r := R.RawExpr("::dafny_runtime::BigInt::from((" + recursiveGen.ToString(IND) + ").borrow().len())");
           } else {
-            s := "::dafny_runtime::BigInt::from(m.borrow().len())";
+            var s := R.RawExpr("::dafny_runtime::BigInt::from(m.borrow().len())").ToString(IND);
             var i := 1;
             while i < dim {
               s := "m.borrow().get(0).map(|m| " + s + ").unwrap_or(::dafny_runtime::BigInt::from(0))";
               i := i + 1;
             }
 
-            s := "(" + recursiveGen + ")" + ".borrow().get(0).map(|m| " + s + ").unwrap_or(::dafny_runtime::BigInt::from(0))";
+            r := R.RcNew(R.RawExpr("(" + recursiveGen.ToString(IND) + ")" + ".borrow().get(0).map(|m| " + s + ").unwrap_or(::dafny_runtime::BigInt::from(0))"));
           }
 
           isOwned := true;
           readIdents := recIdents;
-          isErased := true;
         }
         case SelectFn(on, field, isDatatype, isStatic, arity) => {
-          var onString, onOwned, _, recIdents := GenExpr(on, selfIdent, params, false);
+          var onExpr, onOwned, recIdents := GenExpr(on, selfIdent, params, false);
+          var s: string;
+          var onString := onExpr.ToString(IND);
 
           if isStatic {
             s := onString + "::" + escapeIdent(field);
@@ -2409,24 +2513,24 @@ module {:extern "DCOMP"} DCOMP {
           typeShape := typeShape + ") -> _";
 
           s := "::dafny_runtime::FunctionWrapper(::std::rc::Rc::new(" + s + ") as ::std::rc::Rc<" + typeShape + ">)";
+          r := R.RawExpr(s);
 
           isOwned := true;
-          isErased := false;
           readIdents := recIdents;
         }
         case Select(Companion(c), field, isConstant, isDatatype) => {
-          var onString, onOwned, onErased, recIdents := GenExpr(Companion(c), selfIdent, params, false);
+          var onExpr, onOwned, recIdents := GenExpr(Companion(c), selfIdent, params, false);
 
-          s := onString + "::" + escapeIdent(field) + "()";
+          r := R.RawExpr(onExpr.ToString(IND) + "::" + escapeIdent(field) + "()");
 
           isOwned := true;
-          isErased := false;
           readIdents := recIdents;
         }
         case Select(on, field, isConstant, isDatatype) => {
-          var onString, onOwned, onErased, recIdents := GenExpr(on, selfIdent, params, false);
+          var onExpr, onOwned, recIdents := GenExpr(on, selfIdent, params, false);
+          var s: string;
           if isDatatype || isConstant {
-            s := "(" + onString + ")" + "." + escapeIdent(field) + "()";
+            s := "(" + onExpr.ToString(IND) + ")" + "." + escapeIdent(field) + "()";
             if isConstant {
               s := "&" + s;
             }
@@ -2438,23 +2542,18 @@ module {:extern "DCOMP"} DCOMP {
               isOwned := false;
             }
           } else {
-            s := "::std::ops::Deref::deref(&((" + onString + ")" + "." + escapeIdent(field) + ".borrow()))";
+            s := "::std::ops::Deref::deref(&((" + onExpr.ToString(IND) + ")" + "." + escapeIdent(field) + ".borrow()))";
             s := "(" + s + ").clone()"; // TODO(shadaj): think through when we can avoid cloning
             isOwned := true;
           }
-
-          isErased := false;
+          r := R.RawExpr(s);
           readIdents := recIdents;
         }
         case Index(on, collKind, indices) => {
-          var onString, onOwned, onErased, recIdents := GenExpr(on, selfIdent, params, false);
+          var onExpr, onOwned, recIdents := GenExpr(on, selfIdent, params, false);
           readIdents := recIdents;
-          // if !onErased {
-          //   var eraseFn := if onOwned then "erase_owned" else "erase";
-          //   onString := "::dafny_runtime::DafnyErasable::" + eraseFn + "(" + onString + ")";
-          // }
 
-          s := onString;
+          var s := onExpr.ToString(IND);
 
           var i := 0;
           while i < |indices| {
@@ -2463,16 +2562,13 @@ module {:extern "DCOMP"} DCOMP {
             }
 
             if collKind == CollKind.Map {
-              var idx, idxOwned, idxErased, recIdentsIdx := GenExpr(indices[i], selfIdent, params, false);
-              s := "(" + s + ")[" + (if idxOwned then "&" else "") + idx + "]";
+              var idx, idxOwned, recIdentsIdx := GenExpr(indices[i], selfIdent, params, false);
+              s := "(" + s + ")[" + (if idxOwned then "&" else "") + idx.ToString(IND) + "]";
               readIdents := readIdents + recIdentsIdx;
             } else {
-              var idx, _, idxErased, recIdentsIdx := GenExpr(indices[i], selfIdent, params, true);
-              if !idxErased {
-                idx := "::dafny_runtime::DafnyErasable::erase_owned(" + idx + ")";
-              }
+              var idx, _, recIdentsIdx := GenExpr(indices[i], selfIdent, params, true);
 
-              s := "(" + s + ")[<usize as ::dafny_runtime::NumCast>::from(" + idx + ").unwrap()]";
+              s := "(" + s + ")[<usize as ::dafny_runtime::NumCast>::from(" + idx.ToString(IND) + ").unwrap()]";
               readIdents := readIdents + recIdentsIdx;
             }
 
@@ -2486,22 +2582,18 @@ module {:extern "DCOMP"} DCOMP {
             s := "(&" + s + ")";
             isOwned := false;
           }
-
-          isErased := onErased;
+          r := R.RawExpr(s);
         }
         case IndexRange(on, isArray, low, high) => {
-          var onString, onOwned, onErased, recIdents := GenExpr(on, selfIdent, params, false);
+          var onExpr, onOwned, recIdents := GenExpr(on, selfIdent, params, false);
           readIdents := recIdents;
 
-          s := onString;
+          var s := onExpr.ToString(IND);
 
           var lowString := None;
           match low {
             case Some(l) => {
-              var lString, _, lErased, recIdentsL := GenExpr(l, selfIdent, params, true);
-              if !lErased {
-                lString := "::dafny_runtime::DafnyErasable::erase_owned(" + lString + ")";
-              }
+              var lString, _, recIdentsL := GenExpr(l, selfIdent, params, true);
 
               lowString := Some(lString);
               readIdents := readIdents + recIdentsL;
@@ -2512,10 +2604,7 @@ module {:extern "DCOMP"} DCOMP {
           var highString := None;
           match high {
             case Some(h) => {
-              var hString, _, hErased, recIdentsH := GenExpr(h, selfIdent, params, true);
-              if !hErased {
-                hString := "::dafny_runtime::DafnyErasable::erase_owned(" + hString + ")";
-              }
+              var hString, _, recIdentsH := GenExpr(h, selfIdent, params, true);
 
               highString := Some(hString);
               readIdents := readIdents + recIdentsH;
@@ -2527,22 +2616,25 @@ module {:extern "DCOMP"} DCOMP {
             s := "(" + s + ").borrow()";
           }
 
-          s := "(" + s + ")" + "[" + (match lowString {
-                                        case Some(l) => "<usize as ::dafny_runtime::NumCast>::from(" + l + ").unwrap()"
-                                        case None => ""
-                                      }) + ".." + (match highString {
-                                                     case Some(h) => "<usize as ::dafny_runtime::NumCast>::from(" + h + ").unwrap()"
-                                                     case None => ""
-                                                   }) + "]";
-
-          isErased := onErased;
+          s := "(" + s + ")" + "[" +
+          (
+            match lowString {
+              case Some(l) => "<usize as ::dafny_runtime::NumCast>::from(" + l.ToString(IND) + ").unwrap()"
+              case None => ""
+            })
+          + ".." + (
+            match highString {
+              case Some(h) => "<usize as ::dafny_runtime::NumCast>::from(" + h.ToString(IND) + ").unwrap()"
+              case None => ""
+            }) + "]";
 
           s := "(" + s + ".to_vec())";
+          r := R.RawExpr(s);
           isOwned := true;
         }
         case TupleSelect(on, idx) => {
-          var onString, _, tupErased, recIdents := GenExpr(on, selfIdent, params, false);
-          s := "(" + onString + ")." + Strings.OfNat(idx);
+          var onExpr, _, recIdents := GenExpr(on, selfIdent, params, false);
+          var s := "(" + onExpr.ToString(IND) + ")." + Strings.OfNat(idx);
           if mustOwn {
             s := "(" + s + ")" + ".clone()";
             isOwned := true;
@@ -2550,54 +2642,41 @@ module {:extern "DCOMP"} DCOMP {
             s := "&" + s;
             isOwned := false;
           }
-          isErased := tupErased;
+          r := R.RawExpr(s);
           readIdents := recIdents;
         }
         case Call(on, name, typeArgs, args) => {
           readIdents := {};
 
-          var typeArgString := "";
+          var typeExprs := [];
           if (|typeArgs| >= 1) {
             var typeI := 0;
-            typeArgString := "::<";
             while typeI < |typeArgs| {
-              if typeI > 0 {
-                typeArgString := typeArgString + ", ";
-              }
 
-              var typeString := GenType(typeArgs[typeI], false, false);
-              typeArgString := typeArgString + typeString;
+              var typeExpr := GenType(typeArgs[typeI], false, false);
+              typeExprs := typeExprs + [typeExpr];
 
               typeI := typeI + 1;
             }
-            typeArgString := typeArgString + ">";
           }
 
-          var argString := "";
+          var argExprs := [];
           var i := 0;
           while i < |args| {
-            if i > 0 {
-              argString := argString + ", ";
-            }
-
-            var argExpr, isOwned, argErased, argIdents := GenExpr(args[i], selfIdent, params, false);
+            var argExpr, isOwned, argIdents := GenExpr(args[i], selfIdent, params, false);
             if isOwned {
-              argExpr := "&(" + argExpr + ")";
+              argExpr := R.Borrow(argExpr);
             }
 
-            if !argErased {
-              argExpr := "::dafny_runtime::DafnyErasable::erase(" + argExpr + ")";
-            }
-            argExpr := "::dafny_runtime::DafnyUnerasable::unerase(" + argExpr + ")";
-
-            argString := argString + argExpr;
+            argExprs := argExprs + [argExpr];
             readIdents := readIdents + argIdents;
 
             i := i + 1;
           }
 
-          var enclosingString, _, _, recIdents := GenExpr(on, selfIdent, params, false);
+          var enclosingExpr, _, recIdents := GenExpr(on, selfIdent, params, false);
           readIdents := readIdents + recIdents;
+          var enclosingString := enclosingExpr.ToString(IND);
           match on {
             case Companion(_) => {
               enclosingString := enclosingString + "::" + escapeIdent(name.id);
@@ -2607,9 +2686,8 @@ module {:extern "DCOMP"} DCOMP {
             }
           }
 
-          s := enclosingString + typeArgString + "(" + argString + ")";
+          r := R.Call(R.RawExpr(enclosingString), typeExprs, argExprs);
           isOwned := true;
-          isErased := false;
         }
         case Lambda(params, retType, body) => {
           var paramNames := [];
@@ -2619,7 +2697,7 @@ module {:extern "DCOMP"} DCOMP {
             i := i + 1;
           }
 
-          var recursiveGen, recIdents := GenStmts(body, if selfIdent != None then Some("_this") else None, paramNames, true, "");
+          var recursiveGen, recIdents := GenStmts(body, if selfIdent != None then Some("_this") else None, paramNames, true, R.RawExpr(""));
           readIdents := {};
           var allReadCloned := "";
           while recIdents != {} decreases recIdents {
@@ -2648,16 +2726,15 @@ module {:extern "DCOMP"} DCOMP {
 
             var typStr := GenType(params[i].typ, false, true);
 
-            paramsString := paramsString + escapeIdent(params[i].name) + ": &" + typStr;
-            paramTypes := paramTypes + "&" + typStr;
+            paramsString := paramsString + escapeIdent(params[i].name) + ": " + R.Borrowed(typStr).ToString(IND);
+            paramTypes := paramTypes + R.Borrowed(typStr).ToString(IND);
             i := i + 1;
           }
 
           var retTypeGen := GenType(retType, false, true);
 
-          s := "::dafny_runtime::FunctionWrapper::<::std::rc::Rc<dyn ::std::ops::Fn(" + paramTypes + ") -> " + retTypeGen + ">>({\n" + allReadCloned + "::std::rc::Rc::new(move |" + paramsString + "| -> " + retTypeGen + " {\n" + recursiveGen + "\n})})";
+          r := R.RawExpr("::dafny_runtime::FunctionWrapper::<::std::rc::Rc<dyn ::std::ops::Fn(" + paramTypes + ") -> " + retTypeGen.ToString(IND) + ">>({\n" + allReadCloned + "::std::rc::Rc::new(move |" + paramsString + "| -> " + retTypeGen.ToString(IND) + " {\n" + recursiveGen.ToString(IND) + "\n})})");
           isOwned := true;
-          isErased := false;
         }
         case BetaRedex(values, retType, expr) => {
           var paramNames := [];
@@ -2670,7 +2747,7 @@ module {:extern "DCOMP"} DCOMP {
           }
 
           readIdents := {};
-          s := "{\n";
+          var s := "{\n";
 
           var paramsString := "";
           i := 0;
@@ -2681,41 +2758,34 @@ module {:extern "DCOMP"} DCOMP {
 
             var typStr := GenType(values[i].0.typ, false, true);
 
-            var valueGen, _, valueErased, recIdents := GenExpr(values[i].1, selfIdent, params, true);
-            s := s + "let " + escapeIdent(values[i].0.name) + ": " + typStr + " = ";
+            var valueGen, _, recIdents := GenExpr(values[i].1, selfIdent, params, true);
+            s := s + "let " + escapeIdent(values[i].0.name) + ": " + typStr.ToString(IND) + " = ";
             readIdents := readIdents + recIdents;
-            if valueErased {
-              valueGen := "::dafny_runtime::DafnyUnerasable::<_>::unerase_owned" + "(" + valueGen + ")";
-            }
 
-            s := s + valueGen + ";\n";
+            s := s + valueGen.ToString(IND) + ";\n";
             i := i + 1;
           }
 
-          var recGen, recOwned, recErased, recIdents := GenExpr(expr, selfIdent, paramNames, mustOwn);
+          var recGen, recOwned, recIdents := GenExpr(expr, selfIdent, paramNames, mustOwn);
           readIdents := recIdents - paramNamesSet;
 
-          s := s  + recGen + "\n}";
+          s := s  + recGen.ToString(IND) + "\n}";
+          r := R.RawExpr(s);
           isOwned := recOwned;
-          isErased := recErased;
         }
         case IIFE(name, tpe, value, iifeBody) => {
-          var valueGen, _, valueErased, recIdents := GenExpr(value, selfIdent, params, true);
-          if valueErased {
-            valueGen := "::dafny_runtime::DafnyUnerasable::<_>::unerase_owned" + "(" + valueGen + ")";
-          }
+          var valueGen, _, recIdents := GenExpr(value, selfIdent, params, true);
 
           readIdents := recIdents;
           var valueTypeGen := GenType(tpe, false, true);
-          var bodyGen, _, bodyErased, bodyIdents := GenExpr(iifeBody, selfIdent, params, true);
+          var bodyGen, _, bodyIdents := GenExpr(iifeBody, selfIdent, params, true);
           readIdents := readIdents + (bodyIdents - {name.id});
 
-          s := "{\nlet " + escapeIdent(name.id) + ": " + valueTypeGen + " = " + valueGen + ";\n" + bodyGen + "\n}";
+          r := R.RawExpr("{\nlet " + escapeIdent(name.id) + ": " + valueTypeGen.ToString(IND) + " = " + valueGen.ToString(IND) + ";\n" + bodyGen.ToString(IND) + "\n}");
           isOwned := true;
-          isErased := bodyErased;
         }
         case Apply(func, args) => {
-          var funcString, _, funcErased, recIdents := GenExpr(func, selfIdent, params, false);
+          var funcExpr, _, recIdents := GenExpr(func, selfIdent, params, false);
           readIdents := recIdents;
 
           var argString := "";
@@ -2725,67 +2795,55 @@ module {:extern "DCOMP"} DCOMP {
               argString := argString + ", ";
             }
 
-            var argExpr, isOwned, argErased, argIdents := GenExpr(args[i], selfIdent, params, false);
+            var argExpr, isOwned, argIdents := GenExpr(args[i], selfIdent, params, false);
+            var argExprString := argExpr.ToString(IND);
             if isOwned {
-              argExpr := "&" + argExpr;
+              argExprString := "&" + argExprString;
             }
 
-            argString := argString + argExpr;
+            argString := argString + argExprString;
             readIdents := readIdents + argIdents;
 
             i := i + 1;
           }
 
-          s := "((" + funcString + ").0" + "(" + argString + "))";
+          r := R.RawExpr("((" + funcExpr.ToString(IND) + ").0" + "(" + argString + "))");
           isOwned := true;
-          isErased := false;
         }
         case TypeTest(on, dType, variant) => {
-          var exprGen, _, exprErased, recIdents := GenExpr(on, selfIdent, params, false);
+          var exprGen, _, recIdents := GenExpr(on, selfIdent, params, false);
           var dTypePath := GenPath(dType);
-          s := "matches!(" + exprGen + ".as_ref(), " + dTypePath + "::" + escapeIdent(variant) + "{ .. })";
+          r := R.RawExpr("matches!(" + exprGen.ToString(IND) + ".as_ref(), " + dTypePath + "::" + escapeIdent(variant) + "{ .. })");
           isOwned := true;
-          isErased := true;
           readIdents := recIdents;
         }
         case BoolBoundedPool() => {
-          s := "[false, true]";
+          r := R.RawExpr("[false, true]");
           isOwned := true;
-          isErased := true;
           readIdents := {};
         }
         case SetBoundedPool(of) => {
-          var exprGen, _, exprErased, recIdents := GenExpr(of, selfIdent, params, false);
-          s := "(" + exprGen + ").iter()";
+          var exprGen, _, recIdents := GenExpr(of, selfIdent, params, false);
+          r := R.RawExpr("(" + exprGen.ToString(IND) + ").iter()");
           isOwned := true;
-          isErased := exprErased;
           readIdents := recIdents;
         }
         case SeqBoundedPool(of, includeDuplicates) => {
-          var exprGen, _, exprErased, recIdents := GenExpr(of, selfIdent, params, false);
-          s := "(" + exprGen + ").iter()";
+          var exprGen, _, recIdents := GenExpr(of, selfIdent, params, false);
+          var s := "(" + exprGen.ToString(IND) + ").iter()";
           if !includeDuplicates {
             s := "::dafny_runtime::itertools::Itertools::unique(" + s + ")";
           }
+          r := R.RawExpr(s);
           isOwned := true;
-          isErased := exprErased;
           readIdents := recIdents;
         }
         case IntRange(lo, hi) => {
-          var loString, _, loErased, recIdentsLo := GenExpr(lo, selfIdent, params, true);
-          var hiString, _, hiErased, recIdentsHi := GenExpr(hi, selfIdent, params, true);
+          var lo, _, recIdentsLo := GenExpr(lo, selfIdent, params, true);
+          var hi, _, recIdentsHi := GenExpr(hi, selfIdent, params, true);
 
-          if !loErased {
-            loString := "::dafny_runtime::DafnyErasable::erase_owned(" + loString + ")";
-          }
-
-          if !hiErased {
-            hiString := "::dafny_runtime::DafnyErasable::erase_owned(" + hiString + ")";
-          }
-
-          s := "::dafny_runtime::integer_range(" + loString + ", " + hiString + ")";
+          r := R.RawExpr("::dafny_runtime::integer_range(" + lo.ToString(IND) + ", " + hi.ToString(IND) + ")");
           isOwned := true;
-          isErased := true;
           readIdents := recIdentsLo + recIdentsHi;
         }
       }
